New definition of validity, enforcing Monotonicity. Irrelevance goes through.

theories/Validity.v
@@ -18,12 +18,28 @@ Ltac substitution := eauto with substitution.
   One should think of VRel as a functional relation taking one argument Γ and returning
   2 outputs validSubst and eqSubst *)
 
-  Definition VRel@{i j | i < j +} `{ta : tag} `{!WfContext ta} {wl : wfLCon} :=
+Definition VRel@{i j | i < j +} `{ta : tag} `{!WfContext ta} {wl : wfLCon} :=
     forall
       (Γ : context)
-      (validSubst : forall (Δ : context) (σ : nat -> term) (wfΔ : [|- Δ]< wl >), Type@{i})
-      (eqSubst : forall (Δ : context) (σ σ' : nat -> term) (wfΔ : [|- Δ ]< wl >), validSubst Δ σ wfΔ -> Type@{i})
+      (validSubst : forall (Δ : context) (wl' : wfLCon) (σ : nat -> term)
+                           (f: wl' ≤ε wl) (wfΔ : [|- Δ]< wl' >), Type@{i})
+      (eqSubst : forall (Δ : context) (wl' : wfLCon) (σ σ' : nat -> term) (f : wl' ≤ε wl)
+                        (wfΔ : [|- Δ ]< wl' >), validSubst Δ wl' σ f wfΔ -> Type@{i})
     , Type@{j}.
+
+(*  Definition VRel@{i j | i < j +} `{ta : tag} `{!WfContext ta} {wl : wfLCon} :=
+    forall
+      (Γ : context)
+      (Δ : context)
+      (wl' : wfLCon)
+      (σ : nat -> term)
+      (f : wl' ≤ε wl)
+      (wfΔ : [|- Δ]< wl' >)
+      (validSubst: Type@{i})
+      (eqSubst: (nat -> term) -> validSubst -> Type@{i})
+      
+    , Type@{j}.
+ *)
 
 (* A VPack contains the data corresponding to the codomain of VRel seen as a functional relation *)
 
@@ -31,8 +47,11 @@ Module VPack.
 
   Record VPack@{i} `{ta : tag} `{!WfContext ta} {wl : wfLCon} {Γ : context} :=
   {
-    validSubst : forall (Δ : context) (σ : nat -> term) (wfΔ : [|- Δ]< wl >), Type@{i} ;
-    eqSubst : forall (Δ : context) (σ σ' : nat -> term) (wfΔ : [|- Δ ]< wl >), validSubst Δ σ wfΔ -> Type@{i} ;
+    validSubst : forall (Δ : context) (wl' : wfLCon) (σ : nat -> term)
+                        (f : wl' ≤ε wl) (wfΔ : [|- Δ]< wl' >), Type@{i} ;
+    eqSubst : forall (Δ : context) (wl' : wfLCon) (σ σ': nat -> term)
+                     (f : wl' ≤ε wl) (wfΔ : [|- Δ ]< wl' >),
+      validSubst Δ wl' σ f wfΔ -> Type@{i} ;
   }.
 
   Arguments VPack : clear implicits.
@@ -40,15 +59,19 @@ Module VPack.
   Arguments Build_VPack {_ _}.
 End VPack.
 
+
+
 Export VPack(VPack,Build_VPack).
 
-Notation "[ P | Δ ||-v σ : Γ | wfΔ ]< wl >" := (@VPack.validSubst _ _ wl Γ P Δ σ wfΔ) (at level 0, P, Δ, σ, wl, Γ, wfΔ at level 50).
-Notation "[ P | Δ ||-v σ ≅ σ' : Γ | wfΔ | vσ ]< wl >" := (@VPack.eqSubst _ _ wl Γ P Δ σ σ' wfΔ vσ) (at level 0, P, Δ, σ, σ', wl, Γ, wfΔ, vσ at level 50).
+
+
+Notation "[ P | Δ ||-v σ : Γ | wfΔ | f ]< wl >" := (@VPack.validSubst _ _ wl Γ P Δ _ σ f wfΔ) (at level 0, P, Δ, σ, wl, Γ, wfΔ, f at level 50).
+Notation "[ P | Δ ||-v σ ≅ σ' : Γ | wfΔ | vσ | f ]< wl >" := (@VPack.eqSubst _ _ wl Γ P Δ _ σ σ' f wfΔ vσ) (at level 0, P, Δ, σ, σ', wl, Γ, wfΔ, vσ, f at level 50).
 
 (* An VPack it adequate wrt. a VRel when its three unpacked components are *)
 #[universes(polymorphic)] Definition VPackAdequate@{i j} `{ta : tag} `{!WfContext ta} {wl : wfLCon} {Γ : context}
   (R : VRel@{i j}) (P : VPack@{i} wl Γ) : Type@{j} :=
-  R Γ P.(VPack.validSubst) P.(VPack.eqSubst).
+  R Γ (P.(VPack.validSubst)) (P.(VPack.eqSubst)).
 
 Arguments VPackAdequate _ _ /.
 
@@ -73,8 +96,8 @@ Coercion VAd.pack : VAdequate >-> VPack.
 Coercion VAd.adequate : VAdequate >-> VPackAdequate.
 
 Notation "[ R | ||-v Γ ]< wl >"                            := (VAdequate wl Γ R) (at level 0, R, wl, Γ at level 50).
-Notation "[ R | Δ ||-v σ : Γ | RΓ | wfΔ ]< wl >"           := (RΓ.(@VAd.pack _ _ wl Γ R).(VPack.validSubst) Δ σ wfΔ) (at level 0, R, Δ, σ, wl, Γ, RΓ, wfΔ at level 50).
-Notation "[ R | Δ ||-v σ ≅ σ' : Γ | RΓ | wfΔ | vσ ]< wl >" := (RΓ.(@VAd.pack _ _ wl Γ R).(VPack.eqSubst) Δ σ σ' wfΔ vσ) (at level 0, R, Δ, σ, σ', wl, Γ, RΓ, wfΔ, vσ at level 50).
+Notation "[ R | Δ ||-v σ : Γ | RΓ | wfΔ | f ]< wl >"           := (RΓ.(@VAd.pack _ _ wl Γ R).(VPack.validSubst) Δ _ σ f wfΔ) (at level 0, R, Δ, σ, wl, Γ, RΓ, wfΔ, f at level 50).
+Notation "[ R | Δ ||-v σ ≅ σ' : Γ | RΓ | wfΔ | vσ | f ]< wl >" := (RΓ.(@VAd.pack _ _ wl Γ R).(VPack.eqSubst) Δ _ σ σ' f wfΔ vσ) (at level 0, R, Δ, σ, σ', wl, Γ, RΓ, wfΔ, vσ, f at level 50).
 
 Record typeValidity@{u i j k l} `{ta : tag} `{!WfContext ta}
   `{!WfType ta} `{!Typing ta} `{!ConvType ta}
@@ -82,16 +105,18 @@ Record typeValidity@{u i j k l} `{ta : tag} `{!WfContext ta}
   {wl : wfLCon} {Γ : context} {VΓ : VPack@{u} wl Γ}
   {l : TypeLevel} {A : term} :=
   {
-    validTy : forall {Δ : context} {σ : nat -> term}
-      (wfΔ : [|- Δ ]< wl >)
-      (vσ : [ VΓ | Δ ||-v σ : Γ | wfΔ ]< wl >)
-      , WLogRel@{i j k l} l wl Δ (A [ σ ]);
-    validTyExt : forall {Δ : context} {σ σ' : nat -> term}
-      (wfΔ : [|- Δ ]< wl >)
-      (vσ  : [ VΓ | Δ ||-v σ  : Γ | wfΔ ]< wl >)
-      (vσ' : [ VΓ | Δ ||-v σ' : Γ | wfΔ ]< wl >)
-      (vσσ' : [ VΓ | Δ ||-v σ ≅ σ' : Γ | wfΔ | vσ ]< wl >)
-      , WLogRelEq@{i j k l} l wl Δ (A [ σ ]) (A [ σ' ]) (validTy wfΔ vσ)
+    validTy : forall {Δ : context} {wl': wfLCon} {σ : nat -> term}
+                     (f : wl' ≤ε wl)
+                     (wfΔ : [|- Δ ]< wl' >)
+                     (vσ : [ VΓ | Δ ||-v σ : Γ | wfΔ | f ]< wl >),
+      WLogRel@{i j k l} l wl' Δ (A [ σ ]);
+    validTyExt : forall {Δ : context} {wl': wfLCon} {σ σ' : nat -> term}
+                        (f : wl' ≤ε wl)
+                        (wfΔ : [|- Δ ]< wl' >)
+                        (vσ  : [ VΓ | Δ ||-v σ  : Γ | wfΔ | f ]< wl >)
+                        (vσ' : [ VΓ | Δ ||-v σ' : Γ | wfΔ | f ]< wl >)
+                        (vσσ' : [ VΓ | Δ ||-v σ ≅ σ' : Γ | wfΔ | vσ | f ]< wl >)
+    , WLogRelEq@{i j k l} l wl' Δ (A [ σ ]) (A [ σ' ]) (validTy f wfΔ vσ)
   }.
 
 Arguments typeValidity : clear implicits.
@@ -99,8 +124,15 @@ Arguments typeValidity {_ _ _ _ _ _ _ _ _}.
 
 Notation "[ P | Γ ||-v< l > A ]< wl >" := (typeValidity wl Γ P l A) (at level 0, P, wl, Γ, l, A at level 50).
 
-Definition emptyValidSubst `{ta : tag} `{!WfContext ta} {wl : wfLCon} : forall (Δ : context) (σ : nat -> term) (wfΔ : [|- Δ]< wl >), Type := fun _ _ _ => unit.
-Definition emptyEqSubst@{u} `{ta : tag} `{!WfContext ta} {wl : wfLCon} : forall (Δ : context) (σ σ' : nat -> term) (wfΔ : [|- Δ]< wl >), emptyValidSubst@{u} Δ σ wfΔ -> Type@{u} := fun _ _ _ _ _ => unit.
+
+
+Definition emptyValidSubst `{ta : tag} `{!WfContext ta} {wl : wfLCon} :
+  forall (Δ : context) (wl' : wfLCon) (σ : nat -> term) (f : wl' ≤ε wl) (wfΔ : [|- Δ]< wl' >), Type :=
+  fun _ _ _ _ _ => unit.
+Definition emptyEqSubst@{u} `{ta : tag} `{!WfContext ta} {wl : wfLCon} :
+  forall (Δ : context) (wl' : wfLCon) (σ σ' : nat -> term) (f : wl' ≤ε wl) (wfΔ : [|- Δ]< wl' >),
+    emptyValidSubst@{u} Δ wl' σ f wfΔ -> Type@{u} := fun _ _ _ _ _ _ _ => unit.
+
 Definition emptyVPack `{ta : tag} `{!WfContext ta} {wl : wfLCon} : VPack wl ε :=
   Build_VPack _ _ emptyValidSubst emptyEqSubst.
 
@@ -112,21 +144,45 @@ Section snocValid.
   {wl : wfLCon} {Γ : context} {VΓ : VPack@{u} wl Γ} {A : term} {l : TypeLevel}
   {vA : typeValidity@{u i j k l} wl Γ VΓ l A (* [ VΓ | Γ ||-v< l > A ]< wl > *)}.
 
-  Record snocValidSubst {Δ : context} {σ : nat -> term} {wfΔ : [|- Δ]< wl >} : Type :=
-    {
-      validTail : [ VΓ | Δ ||-v ↑ >> σ : Γ | wfΔ ]< wl > ;
-      validHead : W[ Δ ||-< l > σ var_zero : A[↑ >> σ] | validTy vA wfΔ validTail ]< wl >
+
+  Definition snocValidSubst {Δ : context} {wl' : wfLCon} {σ : nat -> term} {f : wl' ≤ε wl}
+    {wfΔ : [|- Δ]< wl' >} : Type@{u}.
+  Proof.
+    unshelve eapply sigT@{u k}.
+    1: exact [ VΓ | Δ ||-v ↑ >> σ : Γ | wfΔ | f ]< wl >.
+    1: exact (fun validTail => W[ Δ ||-< l > σ var_zero : A[↑ >> σ] | validTy vA f wfΔ validTail ]< wl' >).
+    Defined.
+
+  Arguments snocValidSubst : clear implicits.
+  
+  Definition snocEqSubst {Δ : context} {wl' : wfLCon} {σ σ' : nat -> term} {f : wl' ≤ε wl}
+                 {wfΔ : [|- Δ]< wl' >} {vσ : snocValidSubst Δ wl' σ f wfΔ} : Type@{u}.
+  Proof.
+    unshelve eapply prod@{u k}.
+    - exact [ VΓ | Δ ||-v ↑ >> σ ≅ ↑ >> σ' : Γ | wfΔ | projT1@{u k} vσ | f ]< wl >.
+    - exact (W[ Δ ||-< l > σ var_zero ≅ σ' var_zero : A[↑ >> σ] | validTy vA f wfΔ (projT1@{u k} vσ) ]< wl' >).
+  Defined.
+  
+(*   Record snocValidSubst {Δ : context} {wl' : wfLCon} {σ : nat -> term} {f : wl' ≤ε wl}
+    {wfΔ : [|- Δ]< wl' >} :=
+   { validTail : [ VΓ | Δ ||-v ↑ >> σ : Γ | wfΔ | f ]< wl > ;
+     validHead : W[ Δ ||-< l > σ var_zero : A[↑ >> σ] | validTy vA f wfΔ validTail ]< wl' >
     }.
 
   Arguments snocValidSubst : clear implicits.
 
-  Record snocEqSubst {Δ : context} {σ σ' : nat -> term} {wfΔ : [|- Δ]< wl >} {vσ : snocValidSubst Δ σ wfΔ} : Type :=
+  Record snocEqSubst {Δ : context} {wl' : wfLCon} {σ σ' : nat -> term} {f : wl' ≤ε wl}
+    {wfΔ : [|- Δ]< wl' >} {vσ : snocValidSubst Δ wl' σ f wfΔ} : Type :=
     {
-      eqTail : [ VΓ | Δ ||-v ↑ >> σ ≅ ↑ >> σ' : Γ | wfΔ | validTail vσ ]< wl > ;
-      eqHead : W[ Δ ||-< l > σ var_zero ≅ σ' var_zero : A[↑ >> σ] | validTy vA wfΔ (validTail vσ) ]< wl >
+      eqTail : [ VΓ | Δ ||-v ↑ >> σ ≅ ↑ >> σ' : Γ | wfΔ | validTail vσ | f ]< wl > ;
+      eqHead : W[ Δ ||-< l > σ var_zero ≅ σ' var_zero : A[↑ >> σ] | validTy vA f wfΔ (validTail vσ) ]< wl' >
     }.
+ *)
 
   Definition snocVPack := Build_VPack@{u (* max(u,k) *)} wl (Γ ,, A) snocValidSubst (@snocEqSubst).
+  
+  
+  
 End snocValid.
 
 
@@ -141,23 +197,65 @@ Arguments snocVPack {_ _ _ _ _ _ _ _ _}.
 
 Unset Elimination Schemes.
 
+Definition transport@{k} {A B : Type@{k}} (e : eq A B) (x : A) : B.
+Proof.
+  now destruct e.
+Defined.
+
 Inductive VR@{i j k l} `{ta : tag}
   `{WfContext ta} `{WfType ta} `{Typing ta}
   `{ConvType ta} `{ConvTerm ta} `{ConvNeuConv ta}
-  `{RedType ta} `{RedTerm ta} {wl : wfLCon} : VRel@{k l} :=
-  | VREmpty : VR ε emptyValidSubst@{k} emptyEqSubst@{k}
-  | VRSnoc : forall {Γ A l}
-    (VΓ : VPack@{k} wl Γ)
-    (VΓad : VPackAdequate@{k l} VR VΓ)
-    (VA : typeValidity@{k i j k l} wl Γ VΓ l A (*[ VΓ | Γ ||-v< l > A ]*)),
-    VR (Γ ,, A) (snocValidSubst wl Γ VΓ A l VA) (snocEqSubst wl Γ VΓ A l VA).
+  `{RedType ta} `{RedTerm ta} {wl : wfLCon} : VRel@{k l} (wl := wl)  :=
+| VREmpty : forall (sub : forall Δ wl' σ f wfΔ, Type@{k})
+                  (ext : forall Δ wl' σ σ' f wfΔ Hyp, Type@{k})
+                   (Hsub: forall Δ wl' σ f wfΔ, sub Δ wl' σ f wfΔ = unit)
+                   (Hext : forall Δ wl' σ σ' f wfΔ Hyp, ext Δ wl' σ σ' f wfΔ Hyp = unit),
+    VR ε sub ext
+| VRSnoc : forall {Γ A l} (sub : forall Δ wl' σ f wfΔ, Type@{k})
+                  (ext : forall Δ wl' σ σ' f wfΔ Hyp, Type@{k})
+                  (VΓ : VPack@{k} wl Γ)
+                  (VΓad : VPackAdequate@{k l} VR VΓ)
+                  (VA : typeValidity@{k i j k l} wl Γ VΓ l A (*[ VΓ | Γ ||-v< l > A ]*))
+                  (Hsub: forall Δ wl' σ f wfΔ, sub Δ wl' σ f wfΔ =
+                                                 snocValidSubst _ _ _ _ _ _ Δ wl' σ f wfΔ)
+                  (Hext : forall Δ wl' σ σ' f wfΔ Hyp,
+                      ext Δ wl' σ σ' f wfΔ Hyp =
+                        snocEqSubst _ Γ VΓ _ _ VA Δ wl' σ σ' f wfΔ
+                          (transport (Hsub Δ wl' σ f wfΔ) Hyp)),
+    VR (Γ ,, A) sub ext.
+
+
+(*
+Definition VREmpty'@{i j k l} `{ta : tag}
+  `{WfContext ta} `{WfType ta} `{Typing ta}
+  `{ConvType ta} `{ConvTerm ta} `{ConvNeuConv ta}
+  `{RedType ta} `{RedTerm ta} {wl : wfLCon} : VR@{i j k l} (wl := wl) ε emptyValidSubst@{k} emptyEqSubst.
+Proof.
+  eapply VREmpty.
+  - intros ; now econstructor.
+  - intros ; now econstructor.
+Defined. *)
+
+Definition VRSnoc'@{i j k l} `{ta : tag}
+  `{WfContext ta} `{WfType ta} `{Typing ta}
+  `{ConvType ta} `{ConvTerm ta} `{ConvNeuConv ta}
+  `{RedType ta} `{RedTerm ta} {wl : wfLCon} {Γ A l}
+  (VΓ : VPack@{k} wl Γ)
+  (VΓad : VPackAdequate@{k l} VR@{i j k l} VΓ)
+  (VA : typeValidity@{k i j k l} wl Γ VΓ l A (*[ VΓ | Γ ||-v< l > A ]*)) :
+    VR@{i j k l} (Γ ,, A) (snocValidSubst@{k i j k l} wl Γ VΓ A l VA)
+      (snocEqSubst@{k i j k l} wl Γ VΓ A l VA).
+Proof.
+  intros ; unshelve eapply VRSnoc.
+  all: easy.
+Defined.
 
 
 Set Elimination Schemes.
 
 Notation "[||-v Γ ]< wl >"                             := [ VR | ||-v Γ ]< wl > (at level 0, wl, Γ at level 50).
-Notation "[ Δ ||-v σ : Γ | VΓ | wfΔ ]< wl >"           := [ VR | Δ ||-v σ : Γ | VΓ | wfΔ ]< wl >  (at level 0, Δ, σ, wl, Γ, VΓ, wfΔ at level 50).
-Notation "[ Δ ||-v σ ≅ σ' : Γ | VΓ | wfΔ | vσ ]< wl >" := [ VR | Δ ||-v σ ≅ σ' : Γ | VΓ | wfΔ | vσ ]< wl > (at level 0, Δ, σ, σ', wl, Γ, VΓ, wfΔ, vσ at level 50).
+Notation "[ Δ ||-v σ : Γ | VΓ | wfΔ | f ]< wl >"           := [ VR | Δ ||-v σ : Γ | VΓ | wfΔ | f ]< wl >  (at level 0, Δ, σ, wl, Γ, VΓ, wfΔ, f at level 50).
+Notation "[ Δ ||-v σ ≅ σ' : Γ | VΓ | wfΔ | vσ | f ]< wl >" := [ VR | Δ ||-v σ ≅ σ' : Γ | VΓ | wfΔ | vσ | f ]< wl > (at level 0, Δ, σ, σ', wl, Γ, VΓ, wfΔ, vσ, f at level 50).
 Notation "[ Γ ||-v< l > A | VΓ ]< wl >"                := [ VΓ | Γ ||-v< l > A ]< wl > (at level 0, wl, Γ, l , A, VΓ at level 50).
 
 
@@ -165,44 +263,89 @@ Section MoreDefs.
   Context `{ta : tag} `{WfContext ta} `{WfType ta} `{Typing ta}
   `{ConvType ta} `{ConvTerm ta} `{ConvNeuConv ta} `{RedType ta} `{RedTerm ta}.
 
-  Definition validEmpty@{i j k l} {wl } : [VR@{i j k l}| ||-v ε ]< wl > := Build_VAdequate emptyVPack VREmpty.
+  Definition validEmpty {wl }
+    {sub : forall Δ wl' σ f wfΔ, Type}
+    {ext : forall Δ wl' σ σ' f wfΔ Hyp, Type}
+    (Hsub: forall (Δ : context) (wl' : wfLCon) (σ : nat -> term)
+                  (f : wl' ≤ε wl) (wfΔ : [|- Δ]< wl' >),
+        sub Δ wl' σ f wfΔ = unit)
+    (Hext : forall (Δ : context) (wl' : wfLCon) (σ σ' : nat -> term)
+                   (f : wl' ≤ε wl) (wfΔ : [|- Δ]< wl' >)
+                   (Hyp : sub Δ wl' σ f wfΔ),
+        ext Δ wl' σ σ' f wfΔ Hyp = unit) :
+    [VR| ||-v ε ]< wl >.
+  Proof.
+    unshelve eapply Build_VAdequate.
+    - unshelve econstructor ; assumption.
+    - now eapply VREmpty.
+  Defined.
 
-  Definition validSnoc@{i j k l} {wl Γ} {A l}
-    (VΓ : [VR@{i j k l}| ||-v Γ]< wl >) (VA : [Γ ||-v< l > A | VΓ]< wl >)
-    : [||-v Γ ,, A ]< wl > :=
-    Build_VAdequate (snocVPack wl Γ VΓ A l VA) (VRSnoc VΓ VΓ VA).
+  Definition validSnoc {wl Γ} {A l}
+    (VΓ : [VR| ||-v Γ]< wl >) (VA : (typeValidity wl Γ VΓ l A))
+    {sub : forall Δ wl' σ f wfΔ, Type}
+    {ext : forall Δ wl' σ σ' f wfΔ Hyp, Type}
+    (Hsub: forall (Δ : context) (wl' : wfLCon) (σ : nat -> term)
+                  (f : wl' ≤ε wl) (wfΔ : [|- Δ]< wl' >),
+        sub Δ wl' σ f wfΔ = snocValidSubst _ _ _ _ _ _ Δ wl' σ f wfΔ)
+    (Hext : forall (Δ : context) (wl' : wfLCon) (σ σ' : nat -> term)
+                   (f : wl' ≤ε wl) (wfΔ : [|- Δ]< wl' >)
+                   (Hyp : sub Δ wl' σ f wfΔ),
+        ext Δ wl' σ σ' f wfΔ Hyp =
+          snocEqSubst _ Γ VΓ _ _ VA Δ wl' σ σ' f wfΔ
+            (transport (Hsub Δ wl' σ f wfΔ) Hyp)) :
+    [VR | ||-v Γ ,, A ]< wl >.
+  Proof.
+    unshelve eapply Build_VAdequate.
+    - unshelve econstructor ; assumption.
+    - cbn ; now unshelve eapply (VRSnoc _ _ VΓ VΓ VA). 
+  Defined.
+
+  Definition validSnoc' {wl Γ} {A l}
+    (VΓ : [VR| ||-v Γ]< wl >) (VA : (typeValidity wl Γ VΓ l A)) :
+    [VR | ||-v Γ ,, A ]< wl >.
+  Proof.
+    unshelve eapply Build_VAdequate.
+    - unshelve eapply snocVPack.
+      3: eassumption.
+    - unshelve eapply (VRSnoc _ _ VΓ VΓ VA).
+      1,2: intros ; reflexivity.
+  Defined.
+
 
   Record termValidity@{i j k l} {wl Γ l} {t A : term}
     {VΓ : [VR@{i j k l} (wl := wl) | ||-v Γ]< wl >}
     {VA : typeValidity@{k i j k l} wl Γ VΓ l A (*[Γ ||-v<l> A |VΓ]< wl >*)} : Type :=
     {
-      validTm : forall {Δ σ}
-        (wfΔ : [|- Δ]< wl >) (Vσ : [Δ ||-v σ : Γ | VΓ | wfΔ]< wl >),
-        W[Δ ||-<l> t[σ] : A[σ] | validTy VA wfΔ Vσ ]< wl > ;
-      validTmExt : forall {Δ : context} {σ σ' : nat -> term}
-        (wfΔ : [|- Δ ]< wl >)
-        (Vσ  : [Δ ||-v σ  : Γ | VΓ | wfΔ ]< wl >)
-        (Vσ' : [ Δ ||-v σ' : Γ | VΓ | wfΔ ]< wl >)
-        (Vσσ' : [ Δ ||-v σ ≅ σ' : Γ | VΓ | wfΔ | Vσ ]< wl >),
-        W[Δ ||-<l> t[σ] ≅ t[σ'] : A[σ] | validTy VA wfΔ Vσ ]< wl >
+      validTm : forall {Δ wl' σ} (f : wl' ≤ε wl)
+                       (wfΔ : [|- Δ]< wl' >) (Vσ : [Δ ||-v σ : Γ | VΓ | wfΔ | f ]< wl >),
+        W[Δ ||-<l> t[σ] : A[σ] | validTy VA f wfΔ Vσ ]< wl' > ;
+      validTmExt : forall {Δ : context} {wl' : wfLCon} {σ σ' : nat -> term}
+                          (f : wl' ≤ε wl)
+                          (wfΔ : [|- Δ ]< wl' >)
+                          (Vσ  : [Δ ||-v σ  : Γ | VΓ | wfΔ | f ]< wl >)
+                          (Vσ' : [ Δ ||-v σ' : Γ | VΓ | wfΔ | f ]< wl >)
+                          (Vσσ' : [ Δ ||-v σ ≅ σ' : Γ | VΓ | wfΔ | Vσ | f ]< wl >),
+        W[Δ ||-<l> t[σ] ≅ t[σ'] : A[σ] | validTy VA f wfΔ Vσ ]< wl' >
     }.
 
   Record typeEqValidity@{i j k l} {wl Γ l} {A B : term}
     {VΓ : [VR@{i j k l}| ||-v Γ]< wl >}
     {VA : typeValidity@{k i j k l} wl Γ VΓ l A (*[Γ ||-v<l> A |VΓ]< wl >*)} : Type :=
     {
-      validTyEq : forall {Δ σ}
-        (wfΔ : [|- Δ]< wl >) (Vσ : [Δ ||-v σ : Γ | VΓ | wfΔ]< wl >),
-        W[Δ ||-<l> A[σ] ≅ B[σ] | validTy VA wfΔ Vσ]< wl >
+      validTyEq : forall {Δ wl' σ}
+                          (f : wl' ≤ε wl)
+                          (wfΔ : [|- Δ]< wl' >) (Vσ : [Δ ||-v σ : Γ | VΓ | wfΔ | f ]< wl >),
+        W[Δ ||-<l> A[σ] ≅ B[σ] | validTy VA f wfΔ Vσ]< wl' >
     }.
 
   Record termEqValidity@{i j k l} {wl Γ l} {t u A : term}
     {VΓ : [VR@{i j k l}| ||-v Γ]< wl >}
     {VA : typeValidity@{k i j k l} wl Γ VΓ l A (*[Γ ||-v<l> A |VΓ]< wl >*)} : Type :=
     {
-      validTmEq : forall {Δ σ}
-        (wfΔ : [|- Δ]< wl >) (Vσ : [Δ ||-v σ : Γ | VΓ | wfΔ]< wl >),
-        W[Δ ||-<l> t[σ] ≅ u[σ] : A[σ] | validTy VA wfΔ Vσ]< wl >
+      validTmEq : forall {Δ wl' σ} (f : wl' ≤ε wl)
+                         (wfΔ : [|- Δ]< wl' >)
+                         (Vσ : [Δ ||-v σ : Γ | VΓ | wfΔ | f ]< wl >),
+        W[Δ ||-<l> t[σ] ≅ u[σ] : A[σ] | validTy VA f wfΔ Vσ]< wl' >
     }.
 
   Record tmEqValidity {wl Γ l} {t u A : term} {VΓ : [||-v Γ]< wl >} : Type :=
@@ -215,9 +358,9 @@ Section MoreDefs.
 
   Record redValidity {wl Γ} {t u A : term} {VΓ : [||-v Γ]< wl >} : Type :=
     {
-      validRed : forall {Δ σ}
-        (wfΔ : [|- Δ]< wl >) (Vσ : [Δ ||-v σ : Γ | VΓ | wfΔ]< wl >),
-        [Δ |- t[σ] :⤳*: u[σ] : A[σ]]< wl >
+      validRed : forall {Δ wl' σ} (f : wl' ≤ε wl)
+        (wfΔ : [|- Δ]< wl' >) (Vσ : [Δ ||-v σ : Γ | VΓ | wfΔ | f ]< wl >),
+        [Δ |- t[σ] :⤳*: u[σ] : A[σ]]< wl' >
     }.
 End MoreDefs.
 
@@ -250,32 +393,74 @@ Notation "[ Γ ||-v t :⤳*: u : A | VΓ ]< wl >"      := (redValidity wl Γ t u
 Section Inductions.
   Context `{ta : tag} `{WfContext ta} `{WfType ta} `{Typing ta}
     `{ConvType ta} `{ConvTerm ta} `{ConvNeuConv ta} `{RedType ta} `{RedTerm ta}.
+
+  Set Printing Universes.
+
   
-  Theorem VR_rect {wl}
-    (P : forall {Γ vSubst vSubstExt}, VR Γ vSubst vSubstExt -> Type)
-    (hε : P VREmpty)
-    (hsnoc : forall {Γ A l VΓ VΓad VA},
-      P VΓad -> P (VRSnoc (wl := wl) (Γ := Γ) (A := A) (l := l) VΓ VΓad VA)) :
-    forall {Γ vSubst vSubstExt} (VΓ : VR Γ vSubst vSubstExt), P VΓ.
+  Theorem VR_rect@{h i j k l} {wl : wfLCon}
+    (P : forall {Γ : context}
+                {vSubst}
+                 {vSubstExt},
+        VR@{h i j k} (wl := wl) Γ vSubst vSubstExt -> Type@{l})
+    (hε : forall {vSubst vSubstExt} Hsub Hext,
+        P (VREmpty@{h i j k} vSubst vSubstExt Hsub Hext))
+    (hsnoc : forall {Γ: context} {A l} {vSubst vSubstExt}
+                    (VΓ : VPack@{j} wl Γ) (VΓad : VPackAdequate@{j k} VR@{h i j k} VΓ)
+                    {VA} Hsub Hext,
+        P VΓad ->
+        P (VRSnoc@{h i j k} (A := A) (l := l) vSubst vSubstExt VΓ VΓad VA Hsub Hext)) :
+    forall {Γ : context} {vSubst vSubstExt}
+           (VΓ : VR@{h i j k} Γ vSubst vSubstExt), P VΓ.
   Proof.
     fix ih 4.
-    destruct VΓ; [exact hε | apply hsnoc].
+    destruct VΓ; [eapply hε | apply hsnoc].
     now unshelve eapply ih.
+  Defined.
+
+  
+  Theorem VR_inv {wl Γ vSubst vSubstExt}
+    (VΓ : VR (wl := wl) Γ vSubst vSubstExt) :
+    match Γ as Γ return (VR Γ vSubst vSubstExt)  -> Type with
+    | nil => fun VΓ₀ =>
+               ∑ Hsub Hext, VΓ₀ = VREmpty vSubst vSubstExt Hsub Hext
+    | (A :: Γ)%list => fun (VΓ₀ : VR _ _ _) =>
+                         ∑ l (VΓ' : VPack wl Γ) (VΓad : VPackAdequate VR VΓ')
+      (VA : typeValidity wl Γ VΓ' l A) Hsub Hext,
+      VΓ₀ = VRSnoc (Γ := Γ) (wl := wl) (A := A) vSubst vSubstExt VΓ' VΓad VA Hsub Hext
+    end VΓ .
+  Proof.
+    destruct Γ.
+    1,2: refine (match VΓ with
+            | VREmpty _ _ _ _ => _
+            | VRSnoc _ _ _ _ _ _ _ => _
+              end).
+    2,3: intros X x ; easy. 
+    all: repeat (unshelve eexists _ ; [assumption | ]).
+    all: reflexivity.
   Defined.
 
   Theorem validity_rect {wl}
     (P : forall {Γ : context}, [||-v Γ]< wl > -> Type)
-    (hε : P validEmpty)
-    (hsnoc : forall {Γ A l} (VΓ : [||-v Γ]< wl >) (VA : [Γ ||-v< l > A | VΓ]< wl >), P VΓ -> P (validSnoc VΓ VA)) :
+    (hε : forall sub ext Hsub Hext,
+        P (Γ := ε) (validEmpty (sub := sub) (ext := ext) Hsub Hext))
+    (hsnoc : forall {Γ A l} (VΓ : [||-v Γ]< wl >) (VA : [Γ ||-v< l > A | VΓ]< wl >)
+      sub ext Hsub Hext,
+        P VΓ -> P (validSnoc VΓ VA (sub := sub) (ext := ext) Hsub Hext)) :
     forall {Γ : context} (VΓ : [||-v Γ]< wl >), P VΓ.
   Proof.
+    cbn.
     intros Γ [[s eq] VΓad]; revert Γ s eq VΓad.
+    cbn.
     apply VR_rect.
-    - apply hε.
-    - intros *; apply hsnoc.
+    - cbn ; intros.
+      now apply hε.
+    - intros * Hyp. cbn in *.
+      unshelve eapply hsnoc in Hyp.
+      5,6,7: eassumption.
+      exact Hyp.
   Defined.
-
-  Lemma invValidity {wl Γ} (VΓ : [||-v Γ]< wl >) :
+  
+ (* Lemma invValidity {wl Γ} (VΓ : [||-v Γ]< wl >) :
     match Γ as Γ return [||-v Γ]< wl > -> Type with
     | nil => fun VΓ₀ => VΓ₀ = validEmpty
     | (A :: Γ)%list => fun VΓ₀ =>
@@ -285,23 +470,23 @@ Section Inductions.
     pattern Γ, VΓ. apply validity_rect.
     - reflexivity.
     - intros; do 3 eexists; reflexivity.
-  Qed.
+  Qed. *)
 
-  Lemma invValidityEmpty {wl} (VΓ : [||-v ε]< wl >) : VΓ = validEmpty.
+ (* Lemma invValidityEmpty {wl} (VΓ : [||-v ε]< wl >) : VΓ = validEmpty.
   Proof. apply (invValidity VΓ). Qed.
 
   Lemma invValiditySnoc {wl Γ A} (VΓ₀ : [||-v Γ ,, A ]< wl >) :
       ∑ l (VΓ : [||-v Γ]< wl >) (VA : [Γ ||-v< l > A | VΓ]< wl >), VΓ₀ = validSnoc VΓ VA.
   Proof. apply (invValidity VΓ₀). Qed.
-
+*)
 End Inductions.
 
 (* Tactics to instantiate validity proofs in the context with
   valid substitions *)
 
 Definition wfCtxOfsubstS `{GenericTypingProperties}
-  {wl Γ Δ σ} {VΓ : [||-v Γ]< wl >} {wfΔ : [|- Δ]< wl >} :
-  [Δ ||-v σ : Γ | VΓ | wfΔ]< wl > -> [|- Δ]< wl > := fun _ => wfΔ.
+  {wl Γ Δ wl' σ} {f : wl' ≤ε wl} {VΓ : [||-v Γ]< wl >} {wfΔ : [|- Δ]< wl' >} :
+  [Δ ||-v σ : Γ | VΓ | wfΔ | f ]< wl > -> [|- Δ]< wl' > := fun _ => wfΔ.
 
 Ltac instValid vσ :=
   let wfΔ := (eval unfold wfCtxOfsubstS in (wfCtxOfsubstS vσ)) in
@@ -340,3 +525,55 @@ Ltac instAllValid vσ vσ' vσσ' :=
   instValid vσ ;
   instValid vσ' ;
   instValidExt vσ' vσσ'.
+
+Lemma VPack_Ltrans `{ta : tag} `{!WfContext ta} {wl wl' Γ} : (wl' ≤ε wl) -> VPack wl Γ -> VPack wl' Γ.
+Proof.
+  intros f [H1 H2] ; unshelve econstructor.
+  - intros ? wl'' s f' wfd ; unshelve eapply H1.
+    3,5: eassumption.
+    now eapply wfLCon_le_trans.
+  - intros ? wl'' ?? f' ? Hyp ; cbn in *.
+    unshelve eapply (H2 _ _ σ σ' _ _).
+    5: eassumption.
+Defined.
+
+Lemma Validity_Ltrans `{ta : tag}
+  `{WfContext ta} `{WfType ta} `{Typing ta}
+  `{ConvType ta} `{ConvTerm ta} `{ConvNeuConv ta}
+  `{RedType ta} `{RedTerm ta} {l Γ A wl wl' P} (f: wl' ≤ε wl) :
+  [ P | Γ ||-v< l > A ]< wl > -> [ VPack_Ltrans f P | Γ ||-v< l > A ]< wl' >.
+Proof.
+  intros [red eq] ; unshelve econstructor.
+  - intros ? wl'' ? f' ? Hyp.
+    unshelve eapply red.
+    3: eassumption.
+  - intros ? wl'' ?? f' ????.
+    cbn in *.
+    now unshelve eapply eq.
+Defined.    
+(*
+Lemma test @{i j k l} `{ta : tag}
+  `{WfContext ta} `{WfType ta} `{Typing ta}
+  `{ConvType ta} `{ConvTerm ta} `{ConvNeuConv ta}
+  `{RedType ta} `{RedTerm ta} {wl wl' : wfLCon} (f : wl' ≤ε wl) :
+  forall
+    (Γ : context)
+    (Δ : context)
+    (wl'' : wfLCon)
+    (σ : nat -> term)
+    (f' : wl'' ≤ε wl')
+    (wfΔ : [|- Δ]< wl'' >)
+    (validSubst: Type@{i})
+    (eqSubst: (nat -> term) -> validSubst -> Type@{i}),
+    VR@{i j k l} Γ Δ wl'' σ (f' •ε f) wfΔ validSubst eqSubst ->
+    VR@{i j k l} Γ Δ wl'' σ f' wfΔ validSubst eqSubst.
+Proof.
+  intros * Hyp.
+  induction Hyp as [ | ? ? ? ? wl'' ? f''].
+  - econstructor.
+  - assert ((snocValidSubst@{k i j k l} wl Γ VΓ A l VA Δ wl'' σ f'' wfΔ) =
+              (snocValidSubst@{k i j k l} wl' Γ (VPack_Ltrans f VΓ) A l (Validity_Ltrans f VA) Δ wl'' σ f' wfΔ)).
+    destruct VΓ, VA ; cbn.
+    unfold Validity_Ltrans ; cbn.
+    Set Printing Implicit.
+*)
