theories/Substitution/Conversion.v
@@ -1,6 +1,7 @@
 From LogRel.AutoSubst Require Import core unscoped Ast Extra.
-From LogRel Require Import Utils BasicAst Notations Context NormalForms Weakening GenericTyping LogicalRelation DeclarativeInstance Validity.
+From LogRel Require Import Utils BasicAst Notations LContexts Context NormalForms Weakening GenericTyping LogicalRelation Validity.
 From LogRel.LogicalRelation Require Import Irrelevance Escape Reflexivity Weakening Neutral.
+From LogRel.Substitution Require Import Properties Irrelevance.
 
 Set Universe Polymorphism.
 
@@ -9,12 +10,12 @@ Context `{GenericTypingProperties}.
 
 Set Printing Primitive Projection Parameters.
 
-Lemma conv {Γ t A B l} (VΓ : [||-v Γ])
-  (VA : [Γ ||-v<l> A | VΓ])
-  (VB : [Γ ||-v<l> B | VΓ])
-  (VeqAB : [Γ ||-v<l> A ≅ B | VΓ | VA])
-  (Vt : [Γ ||-v<l> t : A | VΓ | VA]) :
-  [Γ ||-v<l> t : B | VΓ | VB].
+Lemma conv {wl Γ t A B l} (VΓ : [||-v Γ]< wl >)
+  (VA : [Γ ||-v<l> A | VΓ]< wl >)
+  (VB : [Γ ||-v<l> B | VΓ]< wl >)
+  (VeqAB : [Γ ||-v<l> A ≅ B | VΓ | VA]< wl >)
+  (Vt : [Γ ||-v<l> t : A | VΓ | VA]< wl >) :
+  [Γ ||-v<l> t : B | VΓ | VB]< wl >.
 Proof.
   constructor; intros; [eapply LRTmRedConv| eapply LRTmEqRedConv].
   1,3: now unshelve now eapply validTyEq.
@@ -22,12 +23,12 @@ Proof.
   now eapply validTmExt.
 Qed.
 
-Lemma convsym {Γ t A B l} (VΓ : [||-v Γ])
-  (VA : [Γ ||-v<l> A | VΓ])
-  (VB : [Γ ||-v<l> B | VΓ])
-  (VeqAB : [Γ ||-v<l> A ≅ B | VΓ | VA])
-  (Vt : [Γ ||-v<l> t : B | VΓ | VB]) :
-  [Γ ||-v<l> t : A | VΓ | VA].
+Lemma convsym {wl Γ t A B l} (VΓ : [||-v Γ]< wl >)
+  (VA : [Γ ||-v<l> A | VΓ]< wl >)
+  (VB : [Γ ||-v<l> B | VΓ]< wl >)
+  (VeqAB : [Γ ||-v<l> A ≅ B | VΓ | VA]< wl >)
+  (Vt : [Γ ||-v<l> t : B | VΓ | VB]< wl >) :
+  [Γ ||-v<l> t : A | VΓ | VA]< wl >.
 Proof.
   constructor; intros; [eapply LRTmRedConv| eapply LRTmEqRedConv].
   1,3: unshelve eapply LRTyEqSym; tea; [|now unshelve now eapply validTyEq].
@@ -35,16 +36,288 @@ Proof.
   now eapply validTmExt.
 Qed.
 
-Lemma convEq {Γ t u A B l} (VΓ : [||-v Γ])
-  (VA : [Γ ||-v<l> A | VΓ])
-  (VB : [Γ ||-v<l> B | VΓ])
-  (VeqAB : [Γ ||-v<l> A ≅ B | VΓ | VA])
-  (Vt : [Γ ||-v<l> t ≅ u : A | VΓ | VA]) :
-  [Γ ||-v<l> t ≅ u : B | VΓ | VB].
+Lemma convEq {wl Γ t u A B l} (VΓ : [||-v Γ]< wl >)
+  (VA : [Γ ||-v<l> A | VΓ]< wl >)
+  (VB : [Γ ||-v<l> B | VΓ]< wl >)
+  (VeqAB : [Γ ||-v<l> A ≅ B | VΓ | VA]< wl >)
+  (Vt : [Γ ||-v<l> t ≅ u : A | VΓ | VA]< wl >) :
+  [Γ ||-v<l> t ≅ u : B | VΓ | VB]< wl >.
 Proof.
   constructor; intros; eapply LRTmEqRedConv.
   1: now unshelve now eapply validTyEq.
   now eapply validTmEq.
 Qed.
+
+
+Lemma convSubstCtx1 {wl Γ Δ A B l σ} 
+  (VΓ : [||-v Γ]< wl >)
+  (wfΔ : [|- Δ]< wl >)
+  (VΓA : [||-v Γ ,, A]< wl >) 
+  (VΓB : [||-v Γ ,, B]< wl >) 
+  (VA : [_ ||-v<l> A | VΓ]< wl >)
+  (VB : [_ ||-v<l> B | VΓ]< wl >)
+  (VAB : [_ ||-v<l> A ≅ B | VΓ | VA]< wl >)
+  (Vσ : [_ ||-v σ : _ | VΓA | wfΔ]< wl >) :
+  [_ ||-v σ : _ | VΓB | wfΔ]< wl >.
+Proof.
+  pose proof (invValiditySnoc VΓA) as [? [? [?]]]; subst.
+  pose proof (invValiditySnoc VΓB) as [? [? [?]]]; subst.
+  eapply irrelevanceSubstExt.
+  1: rewrite <- scons_eta'; reflexivity.
+  unshelve eapply consSubstS.
+  1: epose (validTail Vσ); irrValid.
+  eapply LRTmRedConv.
+  2: irrelevanceRefl; eapply validHead.
+  now eapply validTyEq.
+  Unshelve. 6: tea.
+    2: eapply irrelevanceSubst; now eapply validTail.
+    tea.
+Qed.
+
+Lemma convSubstEqCtx1 {wl Γ Δ A B l σ σ'} 
+  (VΓ : [||-v Γ]< wl >)
+  (wfΔ : [|- Δ]< wl >)
+  (VΓA : [||-v Γ ,, A]< wl >) 
+  (VΓB : [||-v Γ ,, B]< wl >) 
+  (VA : [_ ||-v<l> A | VΓ]< wl >)
+  (VB : [_ ||-v<l> B | VΓ]< wl >)
+  (VAB : [_ ||-v<l> A ≅ B | VΓ | VA]< wl >)
+  (Vσ : [_ ||-v σ : _ | VΓA | wfΔ]< wl >) 
+  (Vσ' : [_ ||-v σ' : _ | VΓA | wfΔ]< wl >) 
+  (Vσσ' : [_ ||-v σ ≅ σ' : _ | VΓA | wfΔ | Vσ]< wl >) 
+  (VσB : [_ ||-v σ : _ | VΓB | wfΔ]< wl >) :
+  [_ ||-v σ ≅ σ' : _ | VΓB | wfΔ | VσB]< wl >.
+Proof.
+  pose proof (invValiditySnoc VΓA) as [? [? [?]]]; subst.
+  pose proof (invValiditySnoc VΓB) as [? [? [?]]]; subst.
+  eapply irrelevanceSubstEq.
+  eapply irrelevanceSubstEqExt.
+  1: rewrite <- scons_eta'; reflexivity.
+  unshelve eapply consSubstSEq'.
+  8: now eapply eqTail.
+  3: irrValid.
+  3: eapply LRTmEqRedConv.
+  4: now eapply eqHead.
+  2: irrelevanceRefl; eapply validTyEq; irrValid.
+  eapply LRTmRedConv.
+  2: irrelevanceRefl; eapply validHead.
+  eapply validTyExt.
+  1: now eapply validTail.
+  eapply reflSubst.
+  Unshelve.
+  1: now rewrite scons_eta'.
+  9: tea.
+  7: tea.
+  2,6: irrValid.
+  1,2: tea.
+  1,2: eapply irrelevanceSubst; now eapply validTail.
+Qed.
+
+
+Lemma convCtx1 {wl Γ A B P l} 
+  (VΓ : [||-v Γ]< wl >)
+  (VΓA : [||-v Γ ,, A]< wl >) 
+  (VΓB : [||-v Γ ,, B]< wl >) 
+  (VA : [_ ||-v<l> A | VΓ]< wl >)
+  (VB : [_ ||-v<l> B | VΓ]< wl >)
+  (VAB : [_ ||-v<l> A ≅ B | VΓ | VA]< wl >)
+  (VP : [_ ||-v<l> P | VΓA]< wl >) :
+  [_ ||-v<l> P | VΓB]< wl >.
+Proof.
+  opector; intros.
+  - eapply validTy; tea; eapply convSubstCtx1; tea; now eapply symValidTyEq.
+  - irrelevanceRefl; unshelve eapply validTyExt.
+    3,4: tea. 
+    1,2:  eapply convSubstCtx1; tea; now eapply symValidTyEq.
+    eapply convSubstEqCtx1; cycle 2; tea; now eapply symValidTyEq.
+    Unshelve. all: tea.
+Qed.
+
+Lemma convEqCtx1 {wl Γ A B P Q l} 
+  (VΓ : [||-v Γ]< wl >)
+  (VΓA : [||-v Γ ,, A]< wl >) 
+  (VΓB : [||-v Γ ,, B]< wl >) 
+  (VA : [_ ||-v<l> A | VΓ]< wl >)
+  (VB : [_ ||-v<l> B | VΓ]< wl >)
+  (VAB : [_ ||-v<l> A ≅ B | VΓ | VA]< wl >)
+  (VP : [_ ||-v<l> P | VΓA]< wl >)
+  (VPB : [_ ||-v<l> P | VΓB]< wl >)
+  (VPQ : [_ ||-v<l> P ≅ Q | VΓA | VP]< wl >) :
+  [_ ||-v<l> P ≅ Q | VΓB | VPB]< wl >.
+Proof.
+  constructor; intros; irrelevanceRefl.
+  eapply validTyEq; tea.
+  Unshelve. 1: tea. 
+  unshelve eapply convSubstCtx1; cycle 5; tea; now eapply symValidTyEq.
+Qed.
+
+Lemma convSubstCtx2 {wl Γ Δ A1 B1 A2 B2 l σ} 
+  (VΓ : [||-v Γ]< wl >)
+  (wfΔ : [|- Δ]< wl >)
+  (VA1 : [_ ||-v<l> A1 | VΓ]< wl >)
+  (VB1 : [_ ||-v<l> B1 | VΓ]< wl >)
+  (VAB1 : [_ ||-v<l> A1 ≅ B1 | VΓ | VA1]< wl >)
+  (VΓA1 := validSnoc VΓ VA1) 
+  (VΓB1 := validSnoc VΓ VB1) 
+  (VA2 : [_ ||-v<l> A2 | VΓA1]< wl >)
+  (VB2 : [_ ||-v<l> B2 | VΓA1]< wl >)
+  (VAB : [_ ||-v<l> A2 ≅ B2 | VΓA1 | VA2]< wl >)
+  (VB2' := convCtx1 VΓ VΓA1 VΓB1 VA1 VB1 VAB1 VB2)
+  (VΓA12 := validSnoc VΓA1 VA2) 
+  (VΓB12 := validSnoc VΓB1 VB2') 
+  (Vσ : [_ ||-v σ : _ | VΓA12 | wfΔ]< wl >) :
+  [_ ||-v σ : _ | VΓB12 | wfΔ]< wl >.
+Proof.
+  eapply irrelevanceSubstExt.
+  1: rewrite <- scons_eta'; reflexivity.
+  unshelve eapply consSubstS.
+  + eapply convSubstCtx1; tea.
+    now eapply validTail.
+  + eapply LRTmRedConv.
+    2: now eapply validHead.
+    eapply validTyEq; tea.
+  Unshelve. all: tea.
+Qed.
+
+Lemma convSubstCtx2' {wl Γ Δ A1 B1 A2 B2 l σ} 
+  (VΓ : [||-v Γ]< wl >)
+  (wfΔ : [|- Δ]< wl >)
+  (VΓA1 : [||-v Γ ,, A1]< wl >) 
+  (VΓA12 : [||-v Γ ,, A1 ,, A2]< wl >) 
+  (VΓB12 : [||-v Γ ,, B1 ,, B2]< wl >) 
+  (VA1 : [_ ||-v<l> A1 | VΓ]< wl >)
+  (VB1 : [_ ||-v<l> B1 | VΓ]< wl >)
+  (VAB1 : [_ ||-v<l> A1 ≅ B1 | VΓ | VA1]< wl >)
+  (VA2 : [_ ||-v<l> A2 | VΓA1]< wl >)
+  (VB2 : [_ ||-v<l> B2 | VΓA1]< wl >)
+  (VAB : [_ ||-v<l> A2 ≅ B2 | VΓA1 | VA2]< wl >)
+  (Vσ : [_ ||-v σ : _ | VΓA12 | wfΔ]< wl >) :
+  [_ ||-v σ : _ | VΓB12 | wfΔ]< wl >.
+Proof.
+  eapply irrelevanceSubst.
+  eapply convSubstCtx2; irrValid.
+  Unshelve. all: tea; irrValid.
+Qed.
+
+Lemma convSubstEqCtx2 {wl Γ Δ A1 B1 A2 B2 l σ σ'} 
+  (VΓ : [||-v Γ]< wl >)
+  (wfΔ : [|- Δ]< wl >)
+  (VA1 : [_ ||-v<l> A1 | VΓ]< wl >)
+  (VB1 : [_ ||-v<l> B1 | VΓ]< wl >)
+  (VAB1 : [_ ||-v<l> A1 ≅ B1 | VΓ | VA1]< wl >)
+  (VΓA1 := validSnoc VΓ VA1) 
+  (VΓB1 := validSnoc VΓ VB1) 
+  (VA2 : [_ ||-v<l> A2 | VΓA1]< wl >)
+  (VB2 : [_ ||-v<l> B2 | VΓA1]< wl >)
+  (VAB : [_ ||-v<l> A2 ≅ B2 | VΓA1 | VA2]< wl >)
+  (VB2' := convCtx1 VΓ VΓA1 VΓB1 VA1 VB1 VAB1 VB2)
+  (VΓA12 := validSnoc VΓA1 VA2) 
+  (VΓB12 := validSnoc VΓB1 VB2') 
+  (Vσ : [_ ||-v σ : _ | VΓA12 | wfΔ]< wl >) 
+  (Vσ' : [_ ||-v σ' : _ | VΓA12 | wfΔ]< wl >) 
+  (Vσσ' : [_ ||-v σ ≅ σ' : _ | VΓA12 | wfΔ | Vσ]< wl >) 
+  (VσB : [_ ||-v σ : _ | VΓB12 | wfΔ]< wl >) :
+  [_ ||-v σ ≅ σ' : _ | VΓB12 | wfΔ | VσB]< wl >.
+Proof.
+  eapply irrelevanceSubstEq.
+  eapply irrelevanceSubstEqExt.
+  1: rewrite <- scons_eta'; reflexivity.
+  unshelve eapply consSubstSEq'.
+  8:{ eapply convSubstEqCtx1; tea.
+    1: now eapply validTail.
+    now eapply eqTail.
+  }
+  3,4: irrValid.
+  2: eapply convSubstCtx1; tea; now eapply validTail. 
+  3: eapply LRTmEqRedConv.
+  4: now eapply eqHead.
+  2: irrelevanceRefl; eapply validTyEq; irrValid.
+  eapply LRTmRedConv.
+  2: irrelevanceRefl; eapply validHead.
+  eapply validTyExt.
+  1: now eapply validTail.
+  eapply reflSubst.
+  Unshelve.
+  1: now rewrite scons_eta'.
+  11: tea.
+  1,2,6: irrValid.
+  1: tea.
+  2: eapply convSubstCtx1; tea.
+  1,2: now eapply validTail.
+Qed. 
+
+Lemma convSubstEqCtx2' {wl Γ Δ A1 B1 A2 B2 l σ σ'} 
+  (VΓ : [||-v Γ]< wl >)
+  (wfΔ : [|- Δ]< wl >)
+  (VA1 : [_ ||-v<l> A1 | VΓ]< wl >)
+  (VB1 : [_ ||-v<l> B1 | VΓ]< wl >)
+  (VAB1 : [_ ||-v<l> A1 ≅ B1 | VΓ | VA1]< wl >)
+  (VΓA1 : [||-v Γ ,, A1]< wl >) 
+  (VΓB1 : [||-v Γ ,, B1]< wl >) 
+  (VA2 : [_ ||-v<l> A2 | VΓA1]< wl >)
+  (VB2 : [_ ||-v<l> B2 | VΓA1]< wl >)
+  (VAB : [_ ||-v<l> A2 ≅ B2 | VΓA1 | VA2]< wl >)
+  (VB2' : [_ ||-v<l> B2 | VΓB1]< wl >)
+  (VΓA12 : [||-v Γ ,, A1 ,, A2]< wl >) 
+  (VΓB12 : [||-v Γ ,, B1,, B2]< wl >) 
+  (Vσ : [_ ||-v σ : _ | VΓA12 | wfΔ]< wl >) 
+  (Vσ' : [_ ||-v σ' : _ | VΓA12 | wfΔ]< wl >) 
+  (Vσσ' : [_ ||-v σ ≅ σ' : _ | VΓA12 | wfΔ | Vσ]< wl >) 
+  (VσB : [_ ||-v σ : _ | VΓB12 | wfΔ]< wl >) :
+  [_ ||-v σ ≅ σ' : _ | VΓB12 | wfΔ | VσB]< wl >.
+Proof.
+  eapply irrelevanceSubstEq.
+  eapply convSubstEqCtx2; irrValid.
+  Unshelve.  all: tea; irrValid.
+Qed.
+
+Lemma convCtx2 {wl Γ A1 B1 A2 B2 P l} 
+  (VΓ : [||-v Γ]< wl >)
+  (VA1 : [_ ||-v<l> A1 | VΓ]< wl >)
+  (VB1 : [_ ||-v<l> B1 | VΓ]< wl >)
+  (VAB1 : [_ ||-v<l> A1 ≅ B1 | VΓ | VA1]< wl >)
+  (VΓA1 := validSnoc VΓ VA1) 
+  (VΓB1 := validSnoc VΓ VB1) 
+  (VA2 : [_ ||-v<l> A2 | VΓA1]< wl >)
+  (VB2 : [_ ||-v<l> B2 | VΓA1]< wl >)
+  (VAB : [_ ||-v<l> A2 ≅ B2 | VΓA1 | VA2]< wl >)
+  (VB2' := convCtx1 VΓ VΓA1 VΓB1 VA1 VB1 VAB1 VB2)
+  (VΓA12 := validSnoc VΓA1 VA2) 
+  (VΓB12 := validSnoc VΓB1 VB2') 
+  (VP : [_ ||-v<l> P | VΓA12]< wl >) :
+  [_ ||-v<l> P | VΓB12]< wl >.
+Proof.
+  assert [_ ||-v<l> A2 | VΓB1]< wl > by now eapply convCtx1.
+  assert [_ ||-v<l> B1 ≅ A1 | _ | VB1]< wl > by now eapply symValidTyEq.
+  assert [_ ||-v<l> B2 ≅ A2 | _ | VB2']< wl > by (eapply convEqCtx1; tea; now eapply symValidTyEq).
+  opector; intros.
+  - eapply validTy; tea; now eapply convSubstCtx2'.
+  - irrelevanceRefl; unshelve eapply validTyExt.
+    3,4: tea. 
+    1,2:  now eapply convSubstCtx2'.
+    eapply convSubstEqCtx2'; tea.
+    Unshelve. tea.
+Qed.
+
+Lemma convCtx2' {wl Γ A1 A2 B1 B2 P l} 
+  (VΓ : [||-v Γ]< wl >)
+  (VA1 : [_ ||-v<l> A1 | VΓ]< wl >)
+  (VB1 : [_ ||-v<l> B1 | VΓ]< wl >)
+  (VAB1 : [_ ||-v<l> A1 ≅ B1 | VΓ | VA1]< wl >)
+  (VΓA1 : [||-v Γ ,, A1]< wl >) 
+  (VΓB1 : [||-v Γ ,, B1]< wl >) 
+  (VA2 : [_ ||-v<l> A2 | VΓA1]< wl >)
+  (VB2 : [_ ||-v<l> B2 | VΓA1]< wl >)
+  (VAB : [_ ||-v<l> A2 ≅ B2 | VΓA1 | VA2]< wl >)
+  (VB2' : [_ ||-v<l> B2 | VΓB1]< wl >)
+  (VΓA12 : [||-v Γ ,, A1 ,, A2]< wl >) 
+  (VΓB12 : [||-v Γ ,, B1,, B2]< wl >)
+  (VP : [_ ||-v<l> P | VΓA12]< wl >) :
+  [_ ||-v<l> P | VΓB12]< wl >.
+Proof.
+  eapply irrelevanceTy; eapply convCtx2; irrValid.
+  Unshelve. all: tea; irrValid.
+Qed.
+
 
 End Conversion.
