theories/Substitution/Escape.v
@@ -1,6 +1,6 @@
 
 From LogRel.AutoSubst Require Import core unscoped Ast Extra.
-From LogRel Require Import Utils BasicAst Notations Context NormalForms Weakening GenericTyping LogicalRelation DeclarativeInstance Validity.
+From LogRel Require Import Utils BasicAst Notations LContexts Context NormalForms Weakening GenericTyping LogicalRelation Validity.
 From LogRel.LogicalRelation Require Import Irrelevance Escape Reflexivity Weakening Neutral.
 From LogRel.Substitution Require Import Irrelevance Properties.
 
@@ -9,15 +9,15 @@ Set Universe Polymorphism.
 Section Escape.
 Context `{GenericTypingProperties}.
 
-Lemma reducibleTy {Γ l A} (VΓ : [||-v Γ]) (VA : [Γ ||-v<l> A | VΓ]) : [Γ ||-<l> A].
+Lemma reducibleTy {wl Γ l A} (VΓ : [||-v Γ]< wl >) (VA : [Γ ||-v<l> A | VΓ]< wl >) : [Γ ||-<l> A]< wl >.
 Proof.
   replace A with A[tRel] by now asimpl.
   eapply validTy; tea.
   apply idSubstS.
 Qed.
 
-Lemma reducibleTyEq {Γ l A B} (VΓ : [||-v Γ]) (VA : [Γ ||-v<l> A | VΓ]) :
-  [Γ ||-v<l> A ≅ B | VΓ | VA] -> [Γ ||-<l> A ≅ B | reducibleTy VΓ VA].
+Lemma reducibleTyEq {wl Γ l A B} (VΓ : [||-v Γ]< wl >) (VA : [Γ ||-v<l> A | VΓ]< wl >) :
+  [Γ ||-v<l> A ≅ B | VΓ | VA]< wl > -> [Γ ||-<l> A ≅ B | reducibleTy VΓ VA]< wl >.
 Proof.
   intros.
   replace A with A[tRel] by now asimpl.
@@ -26,8 +26,8 @@ Proof.
   irrelevance.
 Qed.
 
-Lemma reducibleTm {Γ l A t} (VΓ : [||-v Γ]) (VA : [Γ ||-v<l> A | VΓ]) : 
-  [Γ ||-v<l> t : A | VΓ | VA] -> [Γ ||-<l> t : A | reducibleTy VΓ VA].
+Lemma reducibleTm {wl Γ l A t} (VΓ : [||-v Γ]< wl >) (VA : [Γ ||-v<l> A | VΓ]< wl >) : 
+  [Γ ||-v<l> t : A | VΓ | VA]< wl > -> [Γ ||-<l> t : A | reducibleTy VΓ VA]< wl >.
 Proof.
   intros.
   replace A with A[tRel] by now asimpl.
@@ -36,8 +36,8 @@ Proof.
   irrelevance.
 Qed.
 
-Lemma reducibleTmEq {Γ l A t u} (VΓ : [||-v Γ]) (VA : [Γ ||-v<l> A | VΓ]) : 
-  [Γ ||-v<l> t ≅ u : A | VΓ | VA] -> [Γ ||-<l> t ≅ u : A | reducibleTy VΓ VA].
+Lemma reducibleTmEq {wl Γ l A t u} (VΓ : [||-v Γ]< wl >) (VA : [Γ ||-v<l> A | VΓ]< wl >) : 
+  [Γ ||-v<l> t ≅ u : A | VΓ | VA]< wl > -> [Γ ||-<l> t ≅ u : A | reducibleTy VΓ VA]< wl >.
 Proof.
   intros.
   replace A with A[tRel] by now asimpl.
@@ -47,28 +47,28 @@ Proof.
   irrelevance.
 Qed.
 
-Lemma escapeTy {Γ l A} (VΓ : [||-v Γ]) (VA : [Γ ||-v<l> A | VΓ]) : [Γ |- A].
+Lemma escapeTy {wl Γ l A} (VΓ : [||-v Γ]< wl >) (VA : [Γ ||-v<l> A | VΓ]< wl >) : [Γ |- A]< wl >.
 Proof. eapply escape; now eapply reducibleTy. Qed.
 
 
-Lemma escapeEq {Γ l A B} (VΓ : [||-v Γ]) (VA : [Γ ||-v<l> A | VΓ]) : 
-  [Γ ||-v<l> A ≅ B | VΓ | VA] -> [Γ |- A ≅ B].
+Lemma escapeEq {wl Γ l A B} (VΓ : [||-v Γ]< wl >) (VA : [Γ ||-v<l> A | VΓ]< wl >) : 
+  [Γ ||-v<l> A ≅ B | VΓ | VA]< wl > -> [Γ |- A ≅ B]< wl >.
 Proof.
   intros; unshelve eapply escapeEq; tea.
   1: now eapply reducibleTy.
   now eapply reducibleTyEq.
 Qed.
 
-Lemma escapeTm {Γ l A t} (VΓ : [||-v Γ]) (VA : [Γ ||-v<l> A | VΓ]) : 
-  [Γ ||-v<l> t : A | VΓ | VA] -> [Γ |- t : A].
+Lemma escapeTm {wl Γ l A t} (VΓ : [||-v Γ]< wl >) (VA : [Γ ||-v<l> A | VΓ]< wl >) : 
+  [Γ ||-v<l> t : A | VΓ | VA]< wl > -> [Γ |- t : A]< wl >.
 Proof.
   intros; unshelve eapply escapeTerm; tea.
   1: now eapply reducibleTy.
   now eapply reducibleTm.
 Qed.
 
-Lemma escapeTmEq {Γ l A t u} (VΓ : [||-v Γ]) (VA : [Γ ||-v<l> A | VΓ]) : 
-  [Γ ||-v<l> t ≅ u : A | VΓ | VA] -> [Γ |- t ≅ u : A].
+Lemma escapeTmEq {wl Γ l A t u} (VΓ : [||-v Γ]< wl >) (VA : [Γ ||-v<l> A | VΓ]< wl >) : 
+  [Γ ||-v<l> t ≅ u : A | VΓ | VA]< wl > -> [Γ |- t ≅ u : A]< wl >.
 Proof.
   intros; unshelve eapply escapeEqTerm; tea.
   1: now eapply reducibleTy.
