theories/Substitution/Irrelevance.v
@@ -1,6 +1,6 @@
 
 From LogRel.AutoSubst Require Import core unscoped Ast Extra.
-From LogRel Require Import Utils BasicAst Notations Context NormalForms Weakening GenericTyping LogicalRelation DeclarativeInstance Validity.
+From LogRel Require Import Utils BasicAst Notations LContexts Context NormalForms Weakening GenericTyping LogicalRelation Validity.
 From LogRel.LogicalRelation Require Import Irrelevance Reflexivity Transitivity.
 
 Set Universe Polymorphism.
@@ -9,266 +9,329 @@ Section Irrelevances.
 Context `{GenericTypingProperties}.
 
 
-Lemma VRirrelevant Γ {vsubst vsubst' veqsubst veqsubst'}
-  (vr : VR Γ vsubst veqsubst) (vr' : VR Γ vsubst' veqsubst') :
-  (forall Δ σ wfΔ wfΔ', vsubst Δ σ wfΔ <~> vsubst' Δ σ wfΔ') ×
-  (forall Δ σ σ' wfΔ wfΔ' vs vs', veqsubst Δ σ σ' wfΔ vs <~> veqsubst' Δ σ σ' wfΔ' vs').
+Lemma VRirrelevant wl Γ {vsubst vsubst' veqsubst veqsubst'}
+  (vr : VR (wl := wl) Γ vsubst veqsubst) (vr' : VR (wl := wl) Γ vsubst' veqsubst') :
+  (forall Δ wl' σ f wfd wfd',
+      vsubst Δ wl' σ f wfd  <~> vsubst' Δ wl' σ f wfd') ×
+    (forall Δ wl' f wfd wfd' σ σ' vs vs',
+        veqsubst Δ wl' σ σ' f wfd vs <~> veqsubst' Δ wl' σ σ' f wfd' vs').
 Proof.
-  revert vsubst' veqsubst' vr'.  pattern Γ, vsubst, veqsubst, vr.
+  revert vsubst' veqsubst' vr'.
+  pattern Γ, vsubst, veqsubst, vr.
   apply VR_rect; clear Γ vsubst veqsubst vr.
-  - intros ?? h. inversion h. split; reflexivity.
-  - intros ?????? ih ?? h. inversion h.
-    specialize (ih _ _ VΓad0); destruct ih as [ih1 ih2].
+  - intros ?????? h.
+    destruct (VR_inv h) as [Hsub' [Hext' eq]] ; subst.
     split.
-    + intros. split; intros []; unshelve econstructor.
-      1,2: eapply ih1; eassumption.
-      1,2: irrelevance.
-    + intros; split; intros []; unshelve econstructor.
-      1,3: eapply ih2; eassumption.
-      1,2: irrelevance.
+    + intros ; split ; intros.
+      * rewrite Hsub'.
+        now econstructor.
+      * rewrite Hsub.
+        now econstructor.
+    + intros ; split ; intros.
+      * rewrite Hext'.
+        now econstructor.
+      * erewrite Hext ; now econstructor.
+  - intros ?????????? ih ?? h.
+    destruct (VR_inv h) as [l' [VΓ' [VΓad' [VA' [Hsub' [Hext' eq]]]]]] ; subst.
+    specialize (ih _ _ VΓad'); destruct ih as [ih1 ih2].
+    split.
+    + intros ; rewrite Hsub', Hsub ; split ; intros [Htail Hhead].
+      all: unshelve econstructor.
+      1,2: eapply ih1 ; eassumption.
+      1,2: now Wirrelevance.
+    + intros ; rewrite Hext, Hext' ; split ; intros [Htail Hhead].
+      all: unshelve econstructor.
+      1,3: eapply ih2 ; eassumption.
+      all: now Wirrelevance.
 Qed.
 
-Lemma irrelevanceSubst {Γ} (VΓ VΓ' : [||-v Γ]) {σ Δ} (wfΔ wfΔ' : [|- Δ]) :
-  [Δ ||-v σ : Γ | VΓ | wfΔ] -> [Δ ||-v σ : Γ | VΓ' | wfΔ'].
+Lemma irrelevanceSubst {wl Γ} (VΓ VΓ' : [||-v Γ]< wl >) {σ Δ wl'} f
+  (wfΔ wfΔ' : [|- Δ]< wl' >) :
+  [Δ ||-v σ : Γ | VΓ | wfΔ | f ]< wl > -> [Δ ||-v σ : Γ | VΓ' | wfΔ' | f ]< wl >.
 Proof.
-  apply (fst (VRirrelevant Γ VΓ.(VAd.adequate) VΓ'.(VAd.adequate))).
+  apply (fst (VRirrelevant wl Γ VΓ.(VAd.adequate) VΓ'.(VAd.adequate))).
 Qed.
 
-Lemma irrelevanceSubstEq {Γ} (VΓ VΓ' : [||-v Γ]) {σ σ' Δ} (wfΔ wfΔ' : [|- Δ])
-  (Vσ : [Δ ||-v σ : Γ | VΓ | wfΔ]) (Vσ' : [Δ ||-v σ : Γ | VΓ' | wfΔ']) :
-  [Δ ||-v σ ≅ σ' : Γ | VΓ | wfΔ | Vσ] -> [Δ ||-v σ ≅ σ' : Γ | VΓ' | wfΔ' | Vσ'].
+Lemma irrelevanceSubstEq {wl Γ} (VΓ VΓ' : [||-v Γ]< wl >) {σ σ' Δ wl'}
+  f (wfΔ wfΔ' : [|- Δ]< wl' >)
+  (Vσ : [Δ ||-v σ : Γ | VΓ | wfΔ | f]< wl >) (Vσ' : [Δ ||-v σ : Γ | VΓ' | wfΔ' | f]< wl >) :
+  [Δ ||-v σ ≅ σ' : Γ | VΓ | wfΔ | Vσ | f]< wl > -> [Δ ||-v σ ≅ σ' : Γ | VΓ' | wfΔ' | Vσ' | f]< wl >.
 Proof.
-  apply (snd (VRirrelevant Γ VΓ.(VAd.adequate) VΓ'.(VAd.adequate))).
+  apply (snd (VRirrelevant wl Γ VΓ.(VAd.adequate) VΓ'.(VAd.adequate))).
 Qed.
 
 Set Printing Primitive Projection Parameters.
 
-Lemma reflSubst {Γ} (VΓ : [||-v Γ]) : forall {σ Δ} (wfΔ : [|- Δ])
-  (Vσ : [Δ ||-v σ : Γ | VΓ | wfΔ]),
-  [Δ ||-v σ ≅ σ : Γ | VΓ | wfΔ | Vσ].
+Lemma reflSubst {wl Γ} (VΓ : [||-v Γ]< wl >) :
+  forall {σ Δ wl'} f (wfΔ : [|- Δ]< wl' >)
+  (Vσ : [Δ ||-v σ : Γ | VΓ | wfΔ | f]< wl >),
+  [Δ ||-v σ ≅ σ : Γ | VΓ | wfΔ | Vσ | f]< wl >.
 Proof.
   pattern Γ, VΓ; apply validity_rect; clear Γ VΓ.
-  - constructor.
-  - intros * ih. unshelve econstructor.
+  - intros.
+    unfold validEmpty ; cbn.
+    rewrite Hext ; now constructor.
+  - intros * ih *. cbn in * ; rewrite Hext.
+    unshelve econstructor.
     1: apply ih.
-    apply LREqTermRefl_. exact (validHead Vσ).
+    apply WreflLRTmEq.
+    revert Vσ.
+    rewrite Hsub ; cbn ; intros [Htail Hhead].
+    exact Hhead.
 Qed.
 
-Lemma symmetrySubstEq {Γ} (VΓ VΓ' : [||-v Γ]) : forall {σ σ' Δ} (wfΔ wfΔ' : [|- Δ])
-  (Vσ : [Δ ||-v σ : Γ | VΓ | wfΔ]) (Vσ' : [Δ ||-v σ' : Γ | VΓ' | wfΔ']),
-  [Δ ||-v σ ≅ σ' : Γ | VΓ | wfΔ | Vσ] -> [Δ ||-v σ' ≅ σ : Γ | VΓ' | wfΔ' | Vσ'].
+Lemma symmetrySubstEq {wl Γ} (VΓ VΓ' : [||-v Γ]< wl >) :
+  forall {σ σ' Δ wl'} f (wfΔ wfΔ' : [|- Δ]< wl' >)
+  (Vσ : [Δ ||-v σ : Γ | VΓ | wfΔ | f]< wl >) (Vσ' : [Δ ||-v σ' : Γ | VΓ' | wfΔ'| f]< wl >),
+    [Δ ||-v σ ≅ σ' : Γ | VΓ | wfΔ | Vσ | f]< wl > ->
+    [Δ ||-v σ' ≅ σ : Γ | VΓ' | wfΔ' | Vσ' | f]< wl >.
 Proof.
   revert VΓ'; pattern Γ, VΓ; apply validity_rect; clear Γ VΓ.
-  - intros VΓ'. rewrite (invValidityEmpty VΓ'). constructor.
-  - intros * ih VΓ'. pose proof (x := invValiditySnoc VΓ').
-    destruct x as [lA'[ VΓ'' [VA' ->]]].
-    intros ????? [tl hd] [tl' hd'] [tleq hdeq].
+  - intros ???? [[vSubst vSubstEq] Vad] * ?.
+    cbn in *.
+    destruct (VR_inv Vad) as [Hsub' [Hext' eq]] ; subst.
+    rewrite Hext' ; constructor.
+  - intros * ih [[vSubst vSubstEq] Vad] *.
+    destruct (VR_inv Vad) as [l' [VΓ' [VΓad' [VA' [Hsub' [Hext' eq]]]]]] ; subst.
+    cbn in *.
+    rewrite Hext, Hext'.
+    revert Vσ ; rewrite (Hsub Δ wl' σ f wfΔ) ; cbn.
+    revert Vσ' ; rewrite (Hsub' Δ wl' σ' f wfΔ') ; cbn.
+    intros [Vtl Vhd] [Vtl' Vhd'] [Htail Hhead].
     unshelve econstructor.
-    1: now eapply ih.
-    eapply LRTmEqSym. cbn in *.
-    revert hdeq. apply LRTmEqRedConv.
+    unshelve eapply ih in Htail ; [now exists VΓ'  | .. ].
+    1: exact wfΔ'.    
+    1: assumption.
+    1: exact Htail.
+    eapply WLRTmEqSym. cbn in *.
+    revert Hhead. apply WLRTmEqRedConv.
     eapply validTyExt. 2:eassumption.
-    eapply irrelevanceSubst; eassumption.
+    now eapply (fst (VRirrelevant wl Γ VΓ.(VAd.adequate) VΓad')).
 Qed.
 
-Lemma transSubstEq {Γ} (VΓ : [||-v Γ]) :
-  forall {σ σ' σ'' Δ} (wfΔ : [|- Δ])
-    (Vσ : [Δ ||-v σ : Γ | VΓ | wfΔ])
-    (Vσ' : [Δ ||-v σ' : Γ | VΓ | wfΔ]),
-    [Δ ||-v σ ≅ σ' : Γ | VΓ | wfΔ | Vσ] ->
-    [Δ ||-v σ' ≅ σ'' : Γ | VΓ | wfΔ | Vσ'] ->
-    [Δ ||-v σ ≅ σ'' : Γ | VΓ | wfΔ | Vσ].
+Lemma transSubstEq {wl Γ} (VΓ : [||-v Γ]< wl >) :
+  forall {σ σ' σ'' Δ wl' f} (wfΔ : [|- Δ]< wl' >)
+    (Vσ : [Δ ||-v σ : Γ | VΓ | wfΔ| f ]< wl >)
+    (Vσ' : [Δ ||-v σ' : Γ | VΓ | wfΔ| f ]< wl >),
+    [Δ ||-v σ ≅ σ' : Γ | VΓ | wfΔ | Vσ| f ]< wl > ->
+    [Δ ||-v σ' ≅ σ'' : Γ | VΓ | wfΔ | Vσ'| f ]< wl > ->
+    [Δ ||-v σ ≅ σ'' : Γ | VΓ | wfΔ | Vσ| f ]< wl >.
 Proof.
   pattern Γ, VΓ; apply validity_rect; clear Γ VΓ.
-  - constructor.
-  - intros * ih * [] []; unshelve econstructor.
+  - intros ; cbn.
+    rewrite Hext ; now constructor.
+  - intros * ih * ; cbn in *.
+    do 3 rewrite Hext.
+    revert Vσ Vσ' ; do 2 rewrite Hsub ; cbn.
+    intros [] [] [] [] ; unshelve econstructor ; cbn in *.
     1: now eapply ih.
-    eapply transEqTerm; tea.
-    eapply LRTmEqRedConv; tea.
-    unshelve eapply LRTyEqSym; tea.
+    eapply WtransEqTerm; tea.
+    eapply WLRTmEqRedConv; tea.
+    unshelve eapply WLRTyEqSym; tea.
     2: unshelve eapply validTyExt.
-    7: eassumption.
-    1: tea.
-    now eapply validTail.
+    7,8,9: eassumption.
+    now tea.
 Qed.
 
-Lemma irrelevanceValidity {Γ} : forall (VΓ VΓ' : [||-v Γ]) {l A},
-  [Γ ||-v<l> A | VΓ] -> [Γ ||-v<l> A | VΓ'].
+Lemma irrelevanceTy {wl Γ} : forall (VΓ VΓ' : [||-v Γ]< wl >) {l A},
+  [Γ ||-v<l> A | VΓ]< wl > -> [Γ ||-v<l> A | VΓ']< wl >.
 Proof.
   intros VΓ VΓ' l A [VA VAext]; unshelve econstructor; intros.
-  - unshelve eapply VA. 2: eapply irrelevanceSubst. all:eassumption.
+  - unshelve eapply VA. 3: eapply irrelevanceSubst. all:eassumption.
   - eapply VAext; [eapply irrelevanceSubst| eapply irrelevanceSubstEq]; eassumption.
 Qed.
 
-
-Lemma irrelevanceLift {l A F G Γ} (VΓ : [||-v Γ])
-  (VF: [Γ ||-v<l> F | VΓ]) (VG: [Γ ||-v<l> G | VΓ])
-  (VFeqG : [Γ ||-v<l> F ≅ G | VΓ | VF]) :
-  [Γ ,, F ||-v<l> A | validSnoc VΓ VF] ->
-  [Γ ,, G ||-v<l> A | validSnoc VΓ VG].
+Lemma irrelevanceTy' {wl Γ Γ' A A' l} (VΓ : [||-v Γ]< wl >) (VΓ' : [||-v Γ']< wl >) (VA : [Γ ||-v<l> A | VΓ]< wl >) : 
+  A = A' -> Γ = Γ' -> [Γ' ||-v<l> A' | VΓ']< wl >.
 Proof.
-  intros [VA VAext]; unshelve econstructor.
-  - intros ??? [hd tl]. eapply VA.
-    unshelve econstructor. 1: eassumption.
-    eapply LRTmRedConv. 2: eassumption.
-    eapply LRTyEqSym; unshelve eapply VFeqG; eassumption.
-  - intros ???? [??] [??] [??]. eapply VAext.
-    + unshelve econstructor. 1: eassumption.
-      eapply LRTmRedConv. 2: eassumption.
-      eapply LRTyEqSym; unshelve eapply VFeqG; eassumption.
-    + unshelve econstructor. 1: eassumption.
-      eapply LRTmEqRedConv. 2: eassumption.
-      eapply LRTyEqSym; unshelve eapply VFeqG; eassumption.
+  intros eqA eqΓ; subst; now eapply irrelevanceTy.
 Qed.
 
-Lemma irrelevanceEq {Γ l A B} (VΓ VΓ' : [||-v Γ]) (VA : [Γ ||-v<l> A | VΓ]) (VA' : [Γ||-v<l> A | VΓ']) :
-  [Γ ||-v< l > A ≅ B | VΓ | VA] -> [Γ ||-v< l > A ≅ B | VΓ' | VA'].
+Lemma irrelevanceLift {l A F G wl Γ} (VΓ : [||-v Γ]< wl >)
+  (VF: [Γ ||-v<l> F | VΓ]< wl >) (VG: [Γ ||-v<l> G | VΓ]< wl >)
+  (VFeqG : [Γ ||-v<l> F ≅ G | VΓ | VF]< wl >) :
+  [Γ ,, F ||-v<l> A | validSnoc' VΓ VF]< wl > ->
+  [Γ ,, G ||-v<l> A | validSnoc' VΓ VG]< wl >.
+Proof.
+  intros [VA VAext]; unshelve econstructor.
+  - intros ????? [hd tl]. eapply VA.
+    unshelve econstructor. 1: eassumption.
+    eapply WLRTmRedConv. 2: eassumption.
+    eapply WLRTyEqSym; unshelve eapply VFeqG; eassumption.
+  - intros ?????? [??] [??] [??]. eapply VAext.
+    + unshelve econstructor. 1: eassumption.
+      eapply WLRTmRedConv. 2: eassumption.
+      eapply WLRTyEqSym; unshelve eapply VFeqG; eassumption.
+    + unshelve econstructor. 1: eassumption.
+      eapply WLRTmEqRedConv. 2: eassumption.
+      eapply WLRTyEqSym; unshelve eapply VFeqG; eassumption.
+Qed.
+
+Lemma irrelevanceTyEq {wl Γ l A B} (VΓ VΓ' : [||-v Γ]< wl >) (VA : [Γ ||-v<l> A | VΓ]< wl >) (VA' : [Γ||-v<l> A | VΓ']< wl >) :
+  [Γ ||-v< l > A ≅ B | VΓ | VA]< wl > -> [Γ ||-v< l > A ≅ B | VΓ' | VA']< wl >.
 Proof.
   intros [h]; constructor; intros.
-  irrelevanceRefl.
-  unshelve apply h. 1:eassumption.
+  Wirrelevance0 ; [reflexivity | ].
+  unshelve apply h. 1,2:eassumption.
   eapply irrelevanceSubst; eassumption.
 Qed.
 
-Lemma irrelevanceEq' {Γ l A A' B} (VΓ VΓ' : [||-v Γ]) (VA : [Γ ||-v<l> A | VΓ]) (VA' : [Γ||-v<l> A' | VΓ']) : A = A' ->
-  [Γ ||-v< l > A ≅ B | VΓ | VA] -> [Γ ||-v< l > A' ≅ B | VΓ' | VA'].
+Lemma irrelevanceTyEq' {wl Γ l A A' B} (VΓ VΓ' : [||-v Γ]< wl >) (VA : [Γ ||-v<l> A | VΓ]< wl >) (VA' : [Γ||-v<l> A' | VΓ']< wl >) : A = A' ->
+  [Γ ||-v< l > A ≅ B | VΓ | VA]< wl > -> [Γ ||-v< l > A' ≅ B | VΓ' | VA']< wl >.
 Proof.
-  intros ->; now eapply irrelevanceEq.
+  intros ->; now eapply irrelevanceTyEq.
 Qed.
 
-Lemma symValidEq {Γ l A B} {VΓ : [||-v Γ]} {VA : [Γ ||-v<l> A | VΓ]} (VB : [Γ ||-v<l> B | VΓ]) :
-  [Γ ||-v<l> A ≅ B | VΓ | VA] -> [Γ ||-v<l> B ≅ A | VΓ | VB].
+Lemma symValidTyEq {wl Γ l A B} {VΓ : [||-v Γ]< wl >} {VA : [Γ ||-v<l> A | VΓ]< wl >} (VB : [Γ ||-v<l> B | VΓ]< wl >) :
+  [Γ ||-v<l> A ≅ B | VΓ | VA]< wl > -> [Γ ||-v<l> B ≅ A | VΓ | VB]< wl >.
 Proof.
   intros; constructor; intros.
-  eapply LRTyEqSym; now eapply validTyEq.
+  eapply WLRTyEqSym; now eapply validTyEq.
   Unshelve. all: tea.
 Qed.
 
-Lemma transValidEq {Γ l A B C} {VΓ : [||-v Γ]}
-  {VA : [Γ ||-v<l> A | VΓ]} {VB : [Γ ||-v<l> B | VΓ]} (VC : [Γ ||-v<l> C | VΓ]):
-  [Γ ||-v<l> A ≅ B | VΓ | VA] -> [Γ ||-v<l> B ≅ C | VΓ | VB] -> [Γ ||-v<l> A ≅ C | VΓ | VA].
+Lemma transValidTyEq {wl Γ l A B C} {VΓ : [||-v Γ]< wl >}
+  {VA : [Γ ||-v<l> A | VΓ]< wl >} {VB : [Γ ||-v<l> B | VΓ]< wl >} :
+  [Γ ||-v<l> A ≅ B | VΓ | VA]< wl > -> [Γ ||-v<l> B ≅ C | VΓ | VB]< wl > -> [Γ ||-v<l> A ≅ C | VΓ | VA]< wl >.
 Proof.
-  constructor; intros; eapply transEq; now eapply validTyEq.
-  Unshelve. all: tea. now eapply validTy.
+  constructor; intros; eapply WLRTransEq; now eapply validTyEq.
+  Unshelve. all: tea.
 Qed.
 
-Lemma irrelevanceTm {Γ l t A} (VΓ VΓ' : [||-v Γ]) (VA : [Γ ||-v<l> A | VΓ]) (VA' : [Γ||-v<l> A | VΓ']) :
-  [Γ ||-v<l> t : A | VΓ | VA] -> [Γ ||-v<l> t : A | VΓ' | VA'].
+Lemma irrelevanceTm'' {wl Γ l l' t A} (VΓ VΓ' : [||-v Γ]< wl >) (VA : [Γ ||-v<l> A | VΓ]< wl >) (VA' : [Γ||-v<l'> A | VΓ']< wl >) :
+  [Γ ||-v<l> t : A | VΓ | VA]< wl > -> [Γ ||-v<l'> t : A | VΓ' | VA']< wl >.
 Proof.
   intros [h1 h2]; unshelve econstructor.
-  - intros. irrelevanceRefl.
-    unshelve apply h1. 1:eassumption.
+  - intros. Wirrelevance0 ; [reflexivity | ].
+    unshelve apply h1. 1,2:eassumption.
     eapply irrelevanceSubst; eassumption.
-  - intros. irrelevanceRefl.
-    unshelve eapply h2. 1: eassumption.
+  - intros. Wirrelevance0 ; [reflexivity | ].
+    unshelve eapply h2. 1,2: eassumption.
     1,2: eapply irrelevanceSubst; eassumption.
     eapply irrelevanceSubstEq; eassumption.
 Qed.
 
-Lemma irrelevanceTm' {Γ l t A A'} (VΓ VΓ' : [||-v Γ]) (VA : [Γ ||-v<l> A | VΓ]) (VA' : [Γ||-v<l> A' | VΓ']) :
-  A = A' -> [Γ ||-v<l> t : A | VΓ | VA] -> [Γ ||-v<l> t : A' | VΓ' | VA'].
+Lemma irrelevanceTm' {wl Γ l l' t A A'} (VΓ VΓ' : [||-v Γ]< wl >) (VA : [Γ ||-v<l> A | VΓ]< wl >) (VA' : [Γ||-v<l'> A' | VΓ']< wl >) :
+  A = A' -> [Γ ||-v<l> t : A | VΓ | VA]< wl > -> [Γ ||-v<l'> t : A' | VΓ' | VA']< wl >.
 Proof.
-  intros ->; now eapply irrelevanceTm.
+  intros ->; now eapply irrelevanceTm''.
 Qed.
 
-Lemma irrelevanceTmLift {l t A F G Γ} (VΓ : [||-v Γ])
-  (VF: [Γ ||-v<l> F | VΓ]) (VG: [Γ ||-v<l> G | VΓ])
-  (VFeqG : [Γ ||-v<l> F ≅ G | VΓ | VF])
-  (VA : [Γ ,, F ||-v<l> A | validSnoc VΓ VF])
-  (VA' : [Γ ,, G ||-v<l> A | validSnoc VΓ VG])  :
-  [Γ ,, F ||-v<l> t : A | validSnoc VΓ VF | VA] ->
-  [Γ ,, G ||-v<l> t : A | validSnoc VΓ VG | VA'].
+Lemma irrelevanceTm {wl Γ l t A} (VΓ VΓ' : [||-v Γ]< wl >) (VA : [Γ ||-v<l> A | VΓ]< wl >) (VA' : [Γ||-v<l> A | VΓ']< wl >) :
+  [Γ ||-v<l> t : A | VΓ | VA]< wl > -> [Γ ||-v<l> t : A | VΓ' | VA']< wl >.
+Proof.
+  now eapply irrelevanceTm''.
+Qed.
+
+
+
+Lemma irrelevanceTmLift {l t A F G wl Γ} (VΓ : [||-v Γ]< wl >)
+  (VF: [Γ ||-v<l> F | VΓ]< wl >) (VG: [Γ ||-v<l> G | VΓ]< wl >)
+  (VFeqG : [Γ ||-v<l> F ≅ G | VΓ | VF]< wl >)
+  (VA : [Γ ,, F ||-v<l> A | validSnoc' VΓ VF]< wl >)
+  (VA' : [Γ ,, G ||-v<l> A | validSnoc' VΓ VG]< wl >)  :
+  [Γ ,, F ||-v<l> t : A | validSnoc' VΓ VF | VA]< wl > ->
+  [Γ ,, G ||-v<l> t : A | validSnoc' VΓ VG | VA']< wl >.
 Proof.
   intros [Vt Vtext]; unshelve econstructor.
-  - intros ??? [hd tl]. irrelevanceRefl. 
+  - intros ????? [hd tl]. Wirrelevance0 ; [reflexivity | ].
     unshelve eapply Vt; tea.
     unshelve econstructor; tea.
-    eapply LRTmRedConv; tea.
-    eapply LRTyEqSym; unshelve eapply VFeqG; eassumption.
-  - intros ???? [??] [??] [??]. irrelevanceRefl. 
+    eapply WLRTmRedConv; tea.
+    eapply WLRTyEqSym; unshelve eapply VFeqG; eassumption.
+  - intros ?????? [??] [??] [??]. Wirrelevance0 ; [reflexivity | ].
     unshelve eapply Vtext; tea.
     + unshelve econstructor; tea.
-      eapply LRTmRedConv; tea.
-      eapply LRTyEqSym; unshelve eapply VFeqG; eassumption.
+      eapply WLRTmRedConv; tea.
+      eapply WLRTyEqSym; unshelve eapply VFeqG; eassumption.
     + unshelve econstructor; tea.
-      eapply LRTmRedConv; tea.
-      eapply LRTyEqSym; unshelve eapply VFeqG; eassumption.
+      eapply WLRTmRedConv; tea.
+      eapply WLRTyEqSym; unshelve eapply VFeqG; eassumption.
     + unshelve econstructor; tea.
-      eapply LRTmEqRedConv; tea.
-      eapply LRTyEqSym; unshelve eapply VFeqG; eassumption.
+      eapply WLRTmEqRedConv; tea.
+      eapply WLRTyEqSym; unshelve eapply VFeqG; eassumption.
 Qed.
 
-Lemma irrelevanceTmEq {Γ l t u A} (VΓ VΓ' : [||-v Γ]) (VA : [Γ ||-v<l> A | VΓ]) (VA' : [Γ||-v<l> A | VΓ']) :
-  [Γ ||-v<l> t ≅ u : A | VΓ | VA] -> [Γ ||-v<l> t ≅ u : A | VΓ' | VA'].
+Lemma irrelevanceTmEq {wl Γ l t u A} (VΓ VΓ' : [||-v Γ]< wl >) (VA : [Γ ||-v<l> A | VΓ]< wl >) (VA' : [Γ||-v<l> A | VΓ']< wl >) :
+  [Γ ||-v<l> t ≅ u : A | VΓ | VA]< wl > -> [Γ ||-v<l> t ≅ u : A | VΓ' | VA']< wl >.
 Proof.
-  intros [h]; constructor; intros; irrelevanceRefl.
+  intros [h]; constructor; intros; Wirrelevance0 ; [reflexivity | ].
   unshelve apply h; tea.
   eapply irrelevanceSubst; eassumption.
 Qed.
 
-Lemma irrelevanceTmEq' {Γ l t u A A'} (VΓ VΓ' : [||-v Γ]) (VA : [Γ ||-v<l> A | VΓ]) (VA' : [Γ||-v<l> A' | VΓ']) :
-  A = A' -> [Γ ||-v<l> t ≅ u : A | VΓ | VA] -> [Γ ||-v<l> t ≅ u : A' | VΓ' | VA'].
+Lemma irrelevanceTmEq' {wl Γ l t u A A'} (VΓ VΓ' : [||-v Γ]< wl >) (VA : [Γ ||-v<l> A | VΓ]< wl >) (VA' : [Γ||-v<l> A' | VΓ']< wl >) :
+  A = A' -> [Γ ||-v<l> t ≅ u : A | VΓ | VA]< wl > -> [Γ ||-v<l> t ≅ u : A' | VΓ' | VA']< wl >.
 Proof.
   intros ->; now eapply irrelevanceTmEq.
 Qed.
 
-Lemma symValidTmEq {Γ l t u A} {VΓ : [||-v Γ]} {VA : [Γ ||-v<l> A | VΓ]} :
-  [Γ ||-v<l> t ≅ u : A| VΓ | VA] -> [Γ ||-v<l> u ≅ t : A | VΓ | VA].
+Lemma symValidTmEq {wl Γ l t u A} {VΓ : [||-v Γ]< wl >} {VA : [Γ ||-v<l> A | VΓ]< wl >} :
+  [Γ ||-v<l> t ≅ u : A| VΓ | VA]< wl > -> [Γ ||-v<l> u ≅ t : A | VΓ | VA]< wl >.
 Proof.
   intros; constructor; intros.
-  eapply LRTmEqSym; now eapply validTmEq.
+  eapply WLRTmEqSym; now eapply validTmEq.
 Qed.
 
-Lemma transValidTmEq {Γ l t u v A} {VΓ : [||-v Γ]}
-  {VA : [Γ ||-v<l> A | VΓ]} :
-  [Γ ||-v<l> t ≅ u : A | VΓ | VA] -> 
-  [Γ ||-v<l> u ≅ v : A | VΓ | VA] -> 
-  [Γ ||-v<l> t ≅ v : A | VΓ | VA].
+Lemma transValidTmEq {wl Γ l t u v A} {VΓ : [||-v Γ]< wl >}
+  {VA : [Γ ||-v<l> A | VΓ]< wl >} :
+  [Γ ||-v<l> t ≅ u : A | VΓ | VA]< wl > -> 
+  [Γ ||-v<l> u ≅ v : A | VΓ | VA]< wl > -> 
+  [Γ ||-v<l> t ≅ v : A | VΓ | VA]< wl >.
 Proof.
-  constructor; intros; eapply transEqTerm; now eapply validTmEq.
+  constructor; intros; eapply WtransEqTerm; now eapply validTmEq.
 Qed.
 
-Lemma irrelevanceSubstExt {Γ} (VΓ : [||-v Γ]) {σ σ' Δ} (wfΔ : [|- Δ]) :
-  σ =1 σ' -> [Δ ||-v σ : Γ | VΓ | wfΔ] -> [Δ ||-v σ' : Γ | VΓ | wfΔ].
+Lemma irrelevanceSubstExt {wl Γ} (VΓ : [||-v Γ]< wl >) {σ σ' Δ wl' f} (wfΔ : [|- Δ]< wl' >) :
+  σ =1 σ' -> [Δ ||-v σ : Γ | VΓ | wfΔ | f]< wl > -> [Δ ||-v σ' : Γ | VΓ | wfΔ | f]< wl >.
 Proof.
   revert σ σ'; pattern Γ, VΓ; apply validity_rect; clear Γ VΓ.
-  - constructor.
-  - intros ????? ih ?? eq.  unshelve econstructor.
-    + eapply ih. 2: now eapply validTail.
+  - intros ; cbn ; rewrite Hsub. now constructor.
+  - intros ????????? ih ?? eq ; cbn ; do 2 rewrite Hsub.
+    intros [Hhead Htail] ; unshelve econstructor.
+    + eapply ih. 2: eassumption.
       now rewrite eq.
     + rewrite <- (eq var_zero).
-      pose proof (validHead X).
-      irrelevance. now rewrite eq.
+      Wirrelevance. now rewrite eq.
 Qed.
 
-Lemma irrelevanceSubstEqExt {Γ} (VΓ : [||-v Γ]) {σ1 σ1' σ2 σ2' Δ}
-  (wfΔ : [|- Δ]) (eq1 : σ1 =1 σ1') (eq2 : σ2 =1 σ2')
-  (Vσ1 : [Δ ||-v σ1 : Γ | VΓ | wfΔ]) :
-  [Δ ||-v σ1 ≅ σ2 : Γ | VΓ | wfΔ | Vσ1] ->
-  [Δ ||-v σ1' ≅ σ2' : Γ | VΓ | wfΔ | irrelevanceSubstExt VΓ wfΔ eq1 Vσ1].
+Lemma irrelevanceSubstEqExt {wl Γ} (VΓ : [||-v Γ]< wl >) {σ1 σ1' σ2 σ2' Δ wl' f}
+  (wfΔ : [|- Δ]< wl' >) (eq1 : σ1 =1 σ1') (eq2 : σ2 =1 σ2')
+  (Vσ1 : [Δ ||-v σ1 : Γ | VΓ | wfΔ| f ]< wl >) :
+  [Δ ||-v σ1 ≅ σ2 : Γ | VΓ | wfΔ | Vσ1| f ]< wl > ->
+  [Δ ||-v σ1' ≅ σ2' : Γ | VΓ | wfΔ | irrelevanceSubstExt VΓ wfΔ eq1 Vσ1| f ]< wl >.
 Proof.
   revert σ1 σ1' σ2 σ2' eq1 eq2 Vσ1; pattern Γ, VΓ; apply validity_rect; clear Γ VΓ.
-  - constructor.
-  - intros ????? ih ???? eq1 eq2 ? X. unshelve econstructor.
+  - intros ; cbn.
+    rewrite (Hext Δ wl' σ1') ; now constructor.
+  - intros ????????? ih ???? eq1 eq2 ? ; cbn in *.
+    rewrite (Hext Δ wl' σ1'), (Hext Δ wl' σ1).
+    intros [Htail Hhead].
+    unshelve econstructor.
     + eapply irrelevanceSubstEq.
       unshelve eapply ih.
-      6: now eapply eqTail.
+      6: eassumption. 
       all: now (rewrite eq1 + rewrite eq2).
-    + rewrite <- (eq1 var_zero); rewrite <- (eq2 var_zero).
-      pose proof (eqHead X).
-      irrelevance.
+    + cbn in *. Wirrelevance0 ; [reflexivity | ].
+      rewrite <- (eq1 var_zero); rewrite <- (eq2 var_zero).
+      Wirrelevance.
       rewrite eq1; reflexivity.
+      Unshelve.
+      2:{ eapply (validTy VA f wfΔ).
+          eapply (transport (Hsub Δ wl' σ1' f wfΔ)
+                    (irrelevanceSubstExt (validSnoc VΓ VA Hsub Hext) wfΔ eq1 Vσ1)).π1.
+      }
 Qed.
 
 End Irrelevances.
 
 Ltac irrValid :=
   match goal with
-  | [_ : _ |- [||-v _]] => idtac
-  | [_ : _ |- [ _ ||-v _ : _ | _ | _]] => eapply irrelevanceSubst
-  | [_ : _ |- [ _ ||-v _ ≅ _ : _ | _ | _ | _]] => eapply irrelevanceSubstEq
-  | [_ : _ |- [_ ||-v<_> _ | _]] => eapply irrelevanceValidity
-  | [_ : _ |- [_ ||-v<_> _ ≅ _ | _ | _]] => eapply irrelevanceEq
-  | [_ : _ |- [_ ||-v<_> _ : _ | _ | _]] => eapply irrelevanceTm
-  | [_ : _ |- [_ ||-v<_> _ ≅ _ : _ | _ | _]] => eapply irrelevanceTmEq
+  | [_ : _ |- [||-v _]< _ >] => idtac
+  | [_ : _ |- [ _ ||-v _ : _ | _ | _| _ ]< _ >] => eapply irrelevanceSubst
+  | [_ : _ |- [ _ ||-v _ ≅ _ : _ | _ | _ | _ | _ ]< _ >] => eapply irrelevanceSubstEq
+  | [_ : _ |- [_ ||-v<_> _ | _]< _ >] => eapply irrelevanceTy
+  | [_ : _ |- [_ ||-v<_> _ ≅ _ | _ | _]< _ >] => eapply irrelevanceTyEq
+  | [_ : _ |- [_ ||-v<_> _ : _ | _ | _]< _ >] => eapply irrelevanceTm
+  | [_ : _ |- [_ ||-v<_> _ ≅ _ : _ | _ | _]< _ >] => eapply irrelevanceTmEq
   end; eassumption.
