theories/Substitution/Monotonicity.v
@@ -1,0 +1,201 @@
+From LogRel.AutoSubst Require Import core unscoped Ast Extra.
+From LogRel Require Import Utils BasicAst Notations LContexts Context NormalForms Weakening GenericTyping LogicalRelation Validity.
+From LogRel.LogicalRelation Require Import Irrelevance Reflexivity Transitivity Monotonicity.
+
+Set Universe Polymorphism.
+
+Section Monotonicity.
+Context `{GenericTypingProperties}.
+
+Lemma VPack_Ltrans {wl wl' Γ} : (wl' ≤ε wl) -> VPack wl Γ -> VPack wl' Γ.
+Proof.
+  intros f [rel Hrel] ; unshelve econstructor.
+  - intros ? wl'' σ f' wfd ; unshelve eapply rel.
+    3,5: eassumption.
+    now eapply wfLCon_le_trans.
+  - intros ? wl'' ?? f' ? Hyp ; cbn in * ; unshelve eapply (Hrel _ _ σ σ' _ _).
+    5: eassumption.
+Defined.
+
+Lemma Validity_Ltrans l Γ A wl wl' (f: wl' ≤ε wl) P :
+  [ P | Γ ||-v< l > A ]< wl > -> [ VPack_Ltrans f P | Γ ||-v< l > A ]< wl' >.
+Proof.
+  intros [red eq] ; unshelve econstructor.
+  - intros ? wl'' ? f' ? Hyp.
+    unshelve eapply red.
+    3: eassumption.
+  - intros ? wl'' ?? f' ????.
+    cbn in *.
+    now unshelve eapply eq.
+Defined.    
+(*
+Lemma VPackAd_Ltrans wl wl' Γ VP
+  (f : wl' ≤ε wl) :
+  VPackAdequate (Γ := Γ) (wl := wl) VR VP ->
+  VPackAdequate (Γ := Γ) (wl := wl') VR (VPack_Ltrans f VP).
+Proof.
+  destruct VP as [red ext] ; cbn in *.
+  induction 1.
+  - constructor 1.
+    + intros ? wl'' ? f' ? ; cbn in * ; now eapply Hsub.
+    + intros ? wl'' ?? f' ?? ; cbn in * ; now eapply Hext.
+  - unshelve econstructor 2 ; cbn in *.
+    1: eassumption.
+    1: eapply VPack_Ltrans ; eauto.
+    1: eapply Validity_Ltrans ; now eauto.
+    all: cbn.
+    2: eassumption.
+    + intros ? wl'' ? f' ?.
+      rewrite Hsub.
+    
+    6: intros ; eapply Hext. eassumption.
+    
+
+    intros HAd ? wl'' ? f' ?.
+  cbn in *.
+  destruct VP as [rel Hrel] ; cbn in *.
+  set (X:= HAd Δ wl'' σ (f' •ε f) wfΔ).
+  Set Printing Implicit.
+  induction X.
+  - now econstructor.
+  - cbn in *.
+    change f0 with (f' •ε f).
+    unshelve econstructor ; cbn in *.
+    2: now eapply VPack_Ltrans.
+    4: eassumption.
+    2: now eapply Validity_Ltrans.
+    + intros ; cbn.
+      erewrite Hsub.
+      destruct  VΓ ; cbn.
+      unfold VPack_Ltrans.
+      f_equal.
+      
+    + intros ? wl'' ? f' ? Hyp ; cbn in *.
+      unshelve econstructor.
+      * now eapply Himpsub.
+      * Wirrelevance0 ; [reflexivity | ].
+  unshelve eapply Himpsub ; [ | | eassumption].
+  + intros ? wl'' ? f' ? Hyp ; cbn in *.
+    eapply Hrevsub.
+    destruct Hyp.
+    unshelve econstructor.
+    eassumption.
+    cbn in *.
+    Wirrelevance.
+  + cbn in * ; intros ? wl'' ?? f'' ? Hyp Hyp2.
+    unshelve econstructor.
+    * now eapply Himpeq.
+    * Wirrelevance0 ; [reflexivity | ].
+  now eapply Himpeq.
+  + cbn in * ; intros ? wl'' ?? f'' ? Hyp Hyp2.
+    eapply Hreveq.
+    destruct Hyp2 ; unshelve econstructor.
+    * assumption.
+    * Wirrelevance.
+Defined.
+*)
+Lemma WfC_Ltrans {wl wl' Γ} : (wl' ≤ε wl) ->
+  [ VR | ||-v Γ ]< wl > ->
+  [ VR | ||-v Γ ]< wl' >.
+Proof.
+  intros f [rel Hrel] ; unshelve econstructor.
+  - now eapply VPack_Ltrans.
+  - cbn in *.
+    destruct rel as [vs eqs] ; cbn in *.
+    induction Hrel.
+    + unshelve econstructor.
+      * intros ; now rewrite Hsub.
+      * intros ; now rewrite Hext. 
+    + unshelve econstructor 2.
+      1: eassumption.
+      1: now eapply VPack_Ltrans.
+      1: now eapply Validity_Ltrans.
+      all: cbn in *.
+      2: eassumption.
+      * intros ; now erewrite Hsub.
+      * intros ; cbn.
+        erewrite Hext.
+        assert ((eq_ind_r
+          (fun T : Type =>
+           T =
+           snocValidSubst wl' Γ (VPack_Ltrans f VΓ) A l (Validity_Ltrans l Γ A wl wl' f VΓ VA) Δ
+             wl'0 σ f0 wfΔ) eq_refl (Hsub Δ wl'0 σ (f0 •ε f) wfΔ)) =
+                  (Hsub Δ wl'0 σ (f0 •ε f) wfΔ)).
+        { generalize ((Hsub Δ wl'0 σ (f0 •ε f) wfΔ)).
+          intros e.
+          refine (match e with
+                  | eq_refl => eq_refl
+                  end).
+        }
+        rewrite <- H10 at 1.
+        reflexivity.
+Defined.        
+
+Lemma Validity_Ltrans'
+  {l Γ A wl wl'} (f: wl' ≤ε wl)
+  (VΓ : [VR (wl := wl) | ||-v Γ]< wl >) :
+  [ Γ ||-v< l > A | VΓ ]< wl > ->
+  [ WfC_Ltrans f VΓ | Γ ||-v< l > A ]< wl' >.
+Proof.
+  intros [red ext] ; unshelve econstructor.
+  - intros ? wl'' ? f' ? Hyp.
+    unshelve eapply red.
+    3: eassumption.
+  - intros ? wl'' ?? f' ????.
+    cbn in *.
+    now unshelve eapply ext.
+Defined.
+
+Arguments Validity_Ltrans [_ _ _ _ _ _ ].
+
+Lemma TmValidity_Ltrans 
+  {l Γ t A wl wl'}
+  (f: wl' ≤ε wl)
+  (VΓ : [VR (wl := wl) | ||-v Γ]< wl >)
+  (VA : [Γ ||-v<l> A |VΓ]< wl >) :
+  [ Γ ||-v< l > t : A | VΓ | VA ]< wl > ->
+  [ Γ ||-v< l > t : A | _ | Validity_Ltrans' f _ VA ]< wl' >.
+Proof.
+  intros [Ht Htext].
+  unshelve econstructor.
+  - intros ? wl'' ? f'' ??.
+    Wirrelevance0 ; [reflexivity | unshelve eapply Ht ].
+    3: eassumption.
+  - intros ? wl'' ?? f'' ?? Hs' Heq.
+    Wirrelevance0 ; [ reflexivity | eapply Htext].
+    + eassumption.
+    + eassumption.
+Qed.
+
+
+Lemma TyEqValidity_Ltrans 
+  {l Γ A B wl wl'}
+  (f: wl' ≤ε wl)
+  (VΓ : [VR (wl := wl) | ||-v Γ]< wl >)
+  (VA : [Γ ||-v<l> A | VΓ]< wl >) :
+  [ Γ ||-v< l > A ≅ B | VΓ | VA ]< wl > ->
+  [ Γ ||-v< l > A ≅ B | _ | Validity_Ltrans' f _ VA ]< wl' >.
+Proof.
+  intros [HB].
+  unshelve econstructor.
+  intros ? wl'' ? f'' ??.
+  Wirrelevance0 ; [reflexivity | unshelve eapply HB ].
+  3: eassumption.
+Qed.
+
+Lemma TmEqValidity_Ltrans 
+  {l Γ t u A wl wl'}
+  (f: wl' ≤ε wl)
+  (VΓ : [VR (wl := wl) | ||-v Γ]< wl >)
+  (VA : [Γ ||-v<l> A | VΓ]< wl >) :
+  [ Γ ||-v< l > t ≅ u : A | VΓ | VA ]< wl > ->
+  [ Γ ||-v< l > t ≅ u : A | _ | Validity_Ltrans' f _ VA ]< wl' >.
+Proof.
+  intros [Htu].
+  unshelve econstructor.
+  intros ? wl'' ? f'' ??.
+  Wirrelevance0 ; [reflexivity | unshelve eapply Htu ].
+  3: eassumption.
+Qed.
+
+End Monotonicity.
