theories/Substitution/SingleSubst.v
@@ -1,6 +1,6 @@
 From LogRel.AutoSubst Require Import core unscoped Ast Extra.
-From LogRel Require Import Utils BasicAst Notations Context NormalForms Weakening GenericTyping LogicalRelation DeclarativeInstance Validity.
-From LogRel.LogicalRelation Require Import Induction Irrelevance Escape Reflexivity Weakening Neutral Transitivity.
+From LogRel Require Import Utils BasicAst Notations LContexts Context NormalForms Weakening GenericTyping Monad LogicalRelation Validity.
+From LogRel.LogicalRelation Require Import Induction Irrelevance Escape Reflexivity Weakening Neutral Monotonicity Transitivity NormalRed.
 From LogRel.Substitution Require Import Irrelevance Properties Conversion.
 
 Set Universe Polymorphism.
@@ -14,11 +14,11 @@ Lemma singleSubstComm G t σ : G[t..][σ] = G[t[σ] .: σ].
 Proof. now asimpl. Qed.
 
 
-Lemma substS {Γ F G t l} {VΓ : [||-v Γ]}
-  {VF : [Γ ||-v<l> F | VΓ]}
-  (VG : [Γ,, F ||-v<l> G | validSnoc VΓ VF])
-  (Vt : [Γ ||-v<l> t : F | VΓ | VF]) :
-  [Γ ||-v<l> G[t..] | VΓ].
+Lemma substS {wl Γ F G t l} {VΓ : [||-v Γ]< wl >}
+  {VF : [Γ ||-v<l> F | VΓ]< wl >}
+  (VG : [Γ,, F ||-v<l> G | validSnoc VΓ VF]< wl >)
+  (Vt : [Γ ||-v<l> t : F | VΓ | VF]< wl >) :
+  [Γ ||-v<l> G[t..] | VΓ]< wl >.
 Proof.
   opector; intros; rewrite singleSubstComm.
   - unshelve eapply validTy. 3,4:  tea.
@@ -30,25 +30,25 @@ Proof.
     Unshelve. all: eassumption.
 Qed.
 
-Lemma substSEq {Γ F F' G G' t t' l} {VΓ : [||-v Γ]} 
-  {VF : [Γ ||-v<l> F | VΓ]}
-  {VF' : [Γ ||-v<l> F' | VΓ]}
-  (VFF' : [Γ ||-v<l> F ≅ F' | VΓ | VF])
+Lemma substSEq {wl Γ F F' G G' t t' l} {VΓ : [||-v Γ]< wl >} 
+  {VF : [Γ ||-v<l> F | VΓ]< wl >}
+  {VF' : [Γ ||-v<l> F' | VΓ]< wl >}
+  (VFF' : [Γ ||-v<l> F ≅ F' | VΓ | VF]< wl >)
   (VΓF := validSnoc VΓ VF)
   (VΓF' := validSnoc VΓ VF')
-  {VG : [Γ,, F ||-v<l> G | VΓF]}
-  (VG' : [Γ,, F' ||-v<l> G' | VΓF'])
-  (VGG' : [Γ ,, F ||-v<l> G ≅ G' | VΓF | VG])
-  (Vt : [Γ ||-v<l> t : F | VΓ | VF])
-  (Vt' : [Γ ||-v<l> t' : F' | VΓ | VF'])
-  (Vtt' : [Γ ||-v<l> t ≅ t' : F | VΓ | VF])
+  {VG : [Γ,, F ||-v<l> G | VΓF]< wl >}
+  (VG' : [Γ,, F' ||-v<l> G' | VΓF']< wl >)
+  (VGG' : [Γ ,, F ||-v<l> G ≅ G' | VΓF | VG]< wl >)
+  (Vt : [Γ ||-v<l> t : F | VΓ | VF]< wl >)
+  (Vt' : [Γ ||-v<l> t' : F' | VΓ | VF']< wl >)
+  (Vtt' : [Γ ||-v<l> t ≅ t' : F | VΓ | VF]< wl >)
   (VGt := substS VG Vt) :
-  [Γ ||-v<l> G[t..] ≅ G'[t'..] | VΓ | VGt].
+  [Γ ||-v<l> G[t..] ≅ G'[t'..] | VΓ | VGt]< wl >.
 Proof.
   constructor; intros.
-  assert (VtF' : [Γ ||-v<l> t : F' | VΓ | VF']) by now eapply conv.
-  pose proof (consSubstSvalid _ _ Vσ _ Vt').
-  pose proof (consSubstSvalid _ _ Vσ _ VtF').
+  assert (VtF' : [Γ ||-v<l> t : F' | VΓ | VF']< wl >) by now eapply conv.
+  pose proof (consSubstSvalid Vσ Vt').
+  pose proof (consSubstSvalid Vσ VtF').
   rewrite singleSubstComm; irrelevance0.
   1: symmetry; apply singleSubstComm.
   eapply transEq.
@@ -60,20 +60,19 @@ Proof.
     eapply validTmEq.
     now eapply convEq.
     Unshelve. all: tea.
-    now eapply validTy.
 Qed.
 
 
 
 
-Lemma substSTm {Γ F G t f l} {VΓ : [||-v Γ]}
-  {VF : [Γ ||-v<l> F | VΓ]}
+Lemma substSTm {wl Γ F G t f l} {VΓ : [||-v Γ]< wl >}
+  {VF : [Γ ||-v<l> F | VΓ]< wl >}
   (VΓF := validSnoc VΓ VF)
-  {VG : [Γ,, F ||-v<l> G | VΓF]}
-  (Vt : [Γ ||-v<l> t : F | VΓ | VF]) 
-  (Vf : [Γ ,, F ||-v<l> f : G | VΓF | VG])
+  {VG : [Γ,, F ||-v<l> G | VΓF]< wl >}
+  (Vt : [Γ ||-v<l> t : F | VΓ | VF]< wl >) 
+  (Vf : [Γ ,, F ||-v<l> f : G | VΓF | VG]< wl >)
   (VGt := substS VG Vt) :
-  [Γ ||-v<l> f[t..] : G[t..] | VΓ | VGt].
+  [Γ ||-v<l> f[t..] : G[t..] | VΓ | VGt]< wl >.
 Proof.
   constructor; intros; rewrite !singleSubstComm; irrelevance0. 
   1,3: symmetry; apply singleSubstComm.
@@ -85,33 +84,33 @@ Proof.
     now apply consSubstSvalid.
 Qed.
 
-Lemma substSTmEq {Γ F F' G G' t t' f f' l} (VΓ : [||-v Γ]) 
-  (VF : [Γ ||-v<l> F | VΓ])
-  (VF' : [Γ ||-v<l> F' | VΓ])
-  (VFF' : [Γ ||-v<l> F ≅ F' | VΓ | VF])
+Lemma substSTmEq {wl Γ F F' G G' t t' f f' l} (VΓ : [||-v Γ]< wl >) 
+  (VF : [Γ ||-v<l> F | VΓ]< wl >)
+  (VF' : [Γ ||-v<l> F' | VΓ]< wl >)
+  (VFF' : [Γ ||-v<l> F ≅ F' | VΓ | VF]< wl >)
   (VΓF := validSnoc VΓ VF)
   (VΓF' := validSnoc VΓ VF')
-  (VG : [Γ,, F ||-v<l> G | VΓF])
-  (VG' : [Γ,, F' ||-v<l> G' | VΓF'])
-  (VGG' : [Γ ,, F ||-v<l> G ≅ G' | VΓF | VG])
-  (Vt : [Γ ||-v<l> t : F | VΓ | VF])
-  (Vt' : [Γ ||-v<l> t' : F' | VΓ | VF'])
-  (Vtt' : [Γ ||-v<l> t ≅ t' : F | VΓ | VF]) 
-  (Vf : [Γ ,, F ||-v<l> f : G | VΓF | VG])
-  (Vf' : [Γ ,, F' ||-v<l> f' : G' | VΓF' | VG'])
-  (Vff' : [Γ ,, F ||-v<l> f ≅ f' : G | VΓF | VG]) :
-  [Γ ||-v<l> f[t..] ≅ f'[t'..] : G[t..] | VΓ | substS VG Vt].
+  (VG : [Γ,, F ||-v<l> G | VΓF]< wl >)
+  (VG' : [Γ,, F' ||-v<l> G' | VΓF']< wl >)
+  (VGG' : [Γ ,, F ||-v<l> G ≅ G' | VΓF | VG]< wl >)
+  (Vt : [Γ ||-v<l> t : F | VΓ | VF]< wl >)
+  (Vt' : [Γ ||-v<l> t' : F' | VΓ | VF']< wl >)
+  (Vtt' : [Γ ||-v<l> t ≅ t' : F | VΓ | VF]< wl >) 
+  (Vf : [Γ ,, F ||-v<l> f : G | VΓF | VG]< wl >)
+  (Vf' : [Γ ,, F' ||-v<l> f' : G' | VΓF' | VG']< wl >)
+  (Vff' : [Γ ,, F ||-v<l> f ≅ f' : G | VΓF | VG]< wl >) :
+  [Γ ||-v<l> f[t..] ≅ f'[t'..] : G[t..] | VΓ | substS VG Vt]< wl >.
 Proof.
   constructor; intros; rewrite !singleSubstComm; irrelevance0. 
   1: symmetry; apply singleSubstComm.
   eapply transEqTerm.
   + unshelve now eapply validTmEq.
     2: now eapply consSubstSvalid.
-  + assert (Vσt : [Δ ||-v (t[σ] .: σ) : _ | VΓF' | wfΔ])
-     by (eapply consValid; tea; now eapply conv).
-    assert (Vσt' : [Δ ||-v (t'[σ] .: σ) : _ | VΓF' | wfΔ])
-     by (eapply consValid; tea; now eapply conv).
-    assert (Vσtσt' : [Δ ||-v (t[σ] .: σ) ≅ (t'[σ] .: σ) : _ | VΓF' | wfΔ | Vσt]).
+  + assert (Vσt : [Δ ||-v (t[σ] .: σ) : _ | VΓF' | wfΔ]< wl >)
+     by (eapply consSubstSvalid; tea; now eapply conv).
+    assert (Vσt' : [Δ ||-v (t'[σ] .: σ) : _ | VΓF' | wfΔ]< wl >)
+     by (eapply consSubstSvalid; tea; now eapply conv).
+    assert (Vσtσt' : [Δ ||-v (t[σ] .: σ) ≅ (t'[σ] .: σ) : _ | VΓF' | wfΔ | Vσt]< wl >).
     1:{
       constructor.
       - bsimpl; epose (reflSubst _  _ Vσ); now eapply irrelevanceSubstEq.
@@ -120,7 +119,7 @@ Proof.
     eapply LRTmEqRedConv.
     2: eapply (validTmExt Vf' _ Vσt Vσt' Vσtσt').
     eapply LRTyEqSym. now eapply validTyEq.
-    Unshelve. 2: now eapply consValid.
+    Unshelve. 2: now eapply consSubstSvalid.
 Qed.
 
 (* Skipping a series of lemmas on single substitution of a weakened term *)
@@ -130,17 +129,17 @@ Lemma liftSubstComm G t σ : G[t]⇑[σ] = G[t[σ] .: ↑ >> σ].
 Proof. now bsimpl. Qed.
 
 
-Lemma substLiftS {Γ F G t l} (VΓ : [||-v Γ])
-  (VF : [Γ ||-v<l> F | VΓ])
+Lemma substLiftS {wl Γ F G t l} (VΓ : [||-v Γ]< wl >)
+  (VF : [Γ ||-v<l> F | VΓ]< wl >)
   (VΓF := validSnoc VΓ VF)
-  (VG : [Γ,, F ||-v<l> G | VΓF])
+  (VG : [Γ,, F ||-v<l> G | VΓF]< wl >)
   (VF' := wk1ValidTy VF VF)
-  (Vt : [Γ,, F ||-v<l> t : F⟨@wk1 Γ F⟩ | VΓF | VF']) :
-  [Γ ,, F ||-v<l> G[t]⇑ | VΓF].
+  (Vt : [Γ,, F ||-v<l> t : F⟨@wk1 Γ F⟩ | VΓF | VF']< wl >) :
+  [Γ ,, F ||-v<l> G[t]⇑ | VΓF]< wl >.
 Proof.
-  assert (h : forall Δ σ (wfΔ: [|- Δ])
-    (vσ: [VΓF | Δ ||-v σ : Γ,, F | wfΔ]),
-    [VΓF | Δ ||-v (t[σ] .: ↑ >> σ) : _ | wfΔ ]).
+  assert (h : forall Δ σ (wfΔ: [|- Δ]< wl >)
+    (vσ: [VΓF | Δ ||-v σ : Γ,, F | wfΔ]< wl >),
+    [VΓF | Δ ||-v (t[σ] .: ↑ >> σ) : _ | wfΔ ]< wl >).
   1:{
     unshelve econstructor.
     + asimpl; now eapply validTail.
@@ -164,18 +163,18 @@ Proof.
       Unshelve. all:tea.
 Qed.
 
-Lemma substLiftSEq {Γ F G G' t l} (VΓ : [||-v Γ])
-  (VF : [Γ ||-v<l> F | VΓ])
+Lemma substLiftSEq {wl Γ F G G' t l} (VΓ : [||-v Γ]< wl >)
+  (VF : [Γ ||-v<l> F | VΓ]< wl >)
   (VΓF := validSnoc VΓ VF)
-  (VG : [Γ,, F ||-v<l> G | VΓF])
-  (VG' : [Γ,, F ||-v<l> G' | VΓF])
-  (VGeq : [Γ,, F ||-v<l> G ≅ G' | VΓF | VG])
+  (VG : [Γ,, F ||-v<l> G | VΓF]< wl >)
+  (VG' : [Γ,, F ||-v<l> G' | VΓF]< wl >)
+  (VGeq : [Γ,, F ||-v<l> G ≅ G' | VΓF | VG]< wl >)
   (VF' := wk1ValidTy VF VF)
-  (Vt : [Γ,, F ||-v<l> t : F⟨@wk1 Γ F⟩ | VΓF | VF']) :
-  [Γ ,, F ||-v<l> G[t]⇑ ≅ G'[t]⇑ | VΓF | substLiftS _ VF VG Vt].
+  (Vt : [Γ,, F ||-v<l> t : F⟨@wk1 Γ F⟩ | VΓF | VF']< wl >) :
+  [Γ ,, F ||-v<l> G[t]⇑ ≅ G'[t]⇑ | VΓF | substLiftS _ VF VG Vt]< wl >.
 Proof.
   constructor; intros; rewrite liftSubstComm.
-  assert (Vσt : [Δ ||-v (t[σ] .: ↑ >> σ) : _ | VΓF | wfΔ ]). 1:{
+  assert (Vσt : [Δ ||-v (t[σ] .: ↑ >> σ) : _ | VΓF | wfΔ ]< wl >). 1:{
     unshelve econstructor.
     + bsimpl. now eapply validTail.
     + bsimpl. instValid Vσ. irrelevance.
@@ -183,69 +182,143 @@ Proof.
   instValid Vσt. irrelevance.
 Qed.
 
-Lemma singleSubstΠ1 {Γ F G t l lF}
-  (ΠFG : [Γ ||-<l> tProd F G])
-  {RF : [Γ ||-<lF> F]}
-  (Rt : [Γ ||-<lF> t : F | RF]) :
-  [Γ ||-<l> G[t..]].
+Lemma substLiftSEq' {wl Γ F G G' t t' l} (VΓ : [||-v Γ]< wl >)
+  (VF : [Γ ||-v<l> F | VΓ]< wl >)
+  (VΓF := validSnoc VΓ VF)
+  (VG : [Γ,, F ||-v<l> G | VΓF]< wl >)
+  (VG' : [Γ,, F ||-v<l> G' | VΓF]< wl >)
+  (VGeq : [Γ,, F ||-v<l> G ≅ G' | VΓF | VG]< wl >)
+  (VF' := wk1ValidTy VF VF)
+  (Vt : [Γ,, F ||-v<l> t : F⟨@wk1 Γ F⟩ | VΓF | VF']< wl >) 
+  (Vt' : [Γ,, F ||-v<l> t' : F⟨@wk1 Γ F⟩ | VΓF | VF']< wl >)
+  (Vtt' : [Γ,, F ||-v<l> t ≅ t' : F⟨@wk1 Γ F⟩ | VΓF | VF']< wl >) :
+  [Γ ,, F ||-v<l> G[t]⇑ ≅ G'[t']⇑ | VΓF | substLiftS _ VF VG Vt]< wl >.
 Proof.
-  apply invLRΠ in ΠFG; destruct ΠFG as [?? red ??? domRed codRed].
-  unshelve eassert (h :=redtywf_whnf red _).
-  1: constructor.
-  symmetry in h; injection h; clear h; intros ;  subst.
+  eapply transValidTyEq.
+  1: eapply substLiftSEq; [| exact VGeq]; tea.
+  constructor; intros; irrelevance0; rewrite liftSubstComm ; [reflexivity|].
+  instValid Vσ.
+  eapply validTyExt.
+  + unshelve eapply consSubstS.
+    6: now eapply validTail.
+    3: exact VF. 
+    irrelevance.
+  + unshelve eapply consSubstSEq'.
+    1: now eapply validTail.
+    1,3: irrelevance.
+    eapply reflSubst.
+    Unshelve. 3: tea. now eapply substLiftS.
+Qed.
+
+
+Lemma singleSubstPoly {wl Γ F G t l lF}
+  (RFG : PolyRed wl Γ l F G)
+  {RF : [Γ ||-<lF> F]< wl >}
+  (Rt : [Γ ||-<lF> t : F | RF]< wl >) :
+  W[Γ ||-<l> G[t..]]< wl >.
+Proof.
   replace G[t..] with G[t .: wk_id (Γ:=Γ) >> tRel] by now bsimpl.
-  unshelve eapply codRed.
-  1: gen_typing.
-  irrelevance0; tea.
+  econstructor ; intros wl' Hover.
+  unshelve eapply (PolyRed.posRed RFG).
+  5: eassumption.
+  2: escape; now gen_typing.
+  1: now eapply wfLCon_le_id.
+  irrelevance0 ; [ | eassumption].
   now bsimpl.
 Qed.
 
-Lemma singleSubstΠ2 {Γ F F' G G' t t' l lF lF'}
-  {ΠFG : [Γ ||-<l> tProd F G]}
-  (ΠFGeq : [Γ ||-<l> tProd F G ≅ tProd F' G' | ΠFG])
-  {RF : [Γ ||-<lF> F]}
-  {RF' : [Γ ||-<lF'> F']}
-  (Rt : [Γ ||-<lF> t : F | RF]) 
-  (Rt' : [Γ ||-<lF'> t' : F' | RF']) 
-  (Rteq : [Γ ||-<lF> t ≅ t' : F | RF])
-  (RGt : [Γ ||-<lF> G[t..]])
-  (RGt' : [Γ ||-<lF'> G'[t'..]]) :
-  [Γ ||-<lF> G[t..] ≅ G'[t'..] | RGt ].
+Lemma singleSubstΠ1 {wl Γ F G t l lF}
+  (ΠFG : [Γ ||-<l> tProd F G]< wl >)
+  {RF : [Γ ||-<lF> F]< wl >}
+  (Rt : [Γ ||-<lF> t : F | RF]< wl >) :
+  W[Γ ||-<l> G[t..]]< wl >.
 Proof.
-  pose (hΠ := invLRΠ ΠFG).
-  assert (heq : [Γ ||-<l> tProd F G ≅ tProd F' G' | LRPi' hΠ]) by irrelevance.
-  destruct hΠ as [?? red ??? domRed codRed codExt]; clear ΠFG ΠFGeq.
-  assert (wfΓ : [|-Γ]) by gen_typing.
-  destruct heq as [?? red' ? domRedEq codRedEq]; cbn in *.
-  unshelve eassert (h :=redtywf_whnf red _).  1: constructor.
-  unshelve eassert (h' :=redtywf_whnf red' _).  1: constructor.
-  symmetry in h; symmetry in h' ; injection h; injection h'; clear h h'; intros ;  subst.
-  assert [Γ ||-<l> t' : F⟨wk_id (Γ:=Γ)⟩ | domRed Γ wk_id wfΓ].
+  eapply singleSubstPoly; tea.
+  eapply (ParamRedTy.polyRed (normRedΠ0 (invLRΠ ΠFG))).
+Qed.
+
+Lemma singleSubstΣ1 {wl Γ F G t l lF}
+  (ΠFG : [Γ ||-<l> tSig F G]< wl >)
+  {RF : [Γ ||-<lF> F]< wl >}
+  (Rt : [Γ ||-<lF> t : F | RF]< wl >) :
+  W[Γ ||-<l> G[t..]]< wl >.
+Proof.
+  eapply singleSubstPoly; tea.
+  eapply (ParamRedTy.polyRed (normRedΣ0 (invLRΣ ΠFG))).
+Qed.
+
+Lemma singleSubstPoly2 {wl Γ F F' G G' t t' l lF lF'}
+  {RFG : PolyRed wl Γ l F G}
+  (RFGeq : PolyRedEq RFG F' G')
+  {RF : [Γ ||-<lF> F]< wl >}
+  {RF' : [Γ ||-<lF'> F']< wl >}
+  (Rt : [Γ ||-<lF> t : F | RF]< wl >) 
+  (Rt' : [Γ ||-<lF'> t' : F' | RF']< wl >) 
+  (Rteq : [Γ ||-<lF> t ≅ t' : F | RF]< wl >)
+  (RGt : W[Γ ||-<lF> G[t..]]< wl >)
+  (RGt' : W[Γ ||-<lF'> G'[t'..]]< wl >) :
+  W[Γ ||-<lF> G[t..] ≅ G'[t'..] | RGt ]< wl >.
+Proof.
+  assert (wfΓ : [|-Γ]< wl >) by (escape ; gen_typing).
+  assert [Γ ||-<l> t' : F⟨wk_id (Γ:=Γ)⟩ | PolyRed.shpRed RFG wk_id (wfLCon_le_id _) wfΓ]< wl >.
   {
     eapply LRTmRedConv; tea.
     eapply LRTyEqSym. 
     replace F' with F'⟨wk_id (Γ := Γ)⟩ by now bsimpl.
-    eapply domRedEq.
+    eapply (PolyRedEq.shpRed RFGeq).
   }
-  eapply transEq.
-  2: (replace G'[t'..] with G'[t' .: wk_id (Γ:=Γ) >> tRel] by now bsimpl); eapply codRedEq.
-  irrelevance0.
-  2: eapply codExt.
-  3: irrelevance0; tea; now bsimpl.
+  eapply WtransEq.
+  2: (replace G'[t'..] with G'[t' .: wk_id (Γ:=Γ) >> tRel] by now bsimpl).
+  2: econstructor ; intros ; irrelevance0 ; [ | unshelve eapply (PolyRedEq.posRed RFGeq wk_id)].
+  econstructor ; intros ; irrelevance0 ; [ | unshelve eapply (PolyRed.posExt (a:= t) RFG wk_id)].
   1: now bsimpl.
-  eassumption.
-  Unshelve. all: tea.
-  irrelevance0; tea; now bsimpl.
+  3,14: eassumption.
+  1,10 : now eapply wfLCon_le_id.
+  2,10: eapply over_tree_fusion_l, over_tree_fusion_l ; exact Hover'.
+  5: eapply over_tree_fusion_l, over_tree_fusion_r ; exact Hover'.
+  5: eapply over_tree_fusion_r, over_tree_fusion_l ; exact Hover'.
+  7: eapply over_tree_fusion_r, over_tree_fusion_r ; exact Hover'.
+  3,6: eassumption.
+  1,2: irrelevance0 ; [ | eassumption] ; now bsimpl.
+  reflexivity.
+  Unshelve.
+  1: now eapply wfLCon_le_id.
+  1: assumption.
+  3-5: now econstructor.
+  2: econstructor ; intros.
+  2: unshelve eapply (PolyRed.posRed RFG).
+  4,5: eassumption.
 Qed.
 
-Lemma substSΠaux {Γ F G t l} 
-  {VΓ : [||-v Γ]}
-  {VF : [Γ ||-v<l> F | VΓ]}
-  (VΠFG : [Γ ||-v<l> tProd F G | VΓ])
-  (Vt : [Γ ||-v<l> t : F | VΓ | VF])
+Lemma singleSubstΠ2 {wl Γ F F' G G' t t' l lF lF'}
+  {ΠFG : [Γ ||-<l> tProd F G]< wl >}
+  (ΠFGeq : [Γ ||-<l> tProd F G ≅ tProd F' G' | ΠFG]< wl >)
+  {RF : [Γ ||-<lF> F]< wl >}
+  {RF' : [Γ ||-<lF'> F']< wl >}
+  (Rt : [Γ ||-<lF> t : F | RF]< wl >) 
+  (Rt' : [Γ ||-<lF'> t' : F' | RF']< wl >) 
+  (Rteq : [Γ ||-<lF> t ≅ t' : F | RF]< wl >)
+  (RGt : W[Γ ||-<lF> G[t..]]< wl >)
+  (RGt' : W[Γ ||-<lF'> G'[t'..]]< wl >) :
+  W[Γ ||-<lF> G[t..] ≅ G'[t'..] | RGt ]< wl >.
+Proof.
+  eapply singleSubstPoly2; tea.
+  pose (hΠ := normRedΠ0 (invLRΠ ΠFG)).
+  assert (heq : [Γ ||-<l> tProd F G ≅ tProd F' G' | LRPi' hΠ]< wl >) by irrelevance.
+  destruct heq as [?? red' ?? polyRed]; cbn in *.
+  assert (h' :=redtywf_whnf red' whnf_tProd).
+  symmetry in h'; injection h'; clear h'; intros ;  subst.
+  exact polyRed.
+Qed.
+
+Lemma substSΠaux {wl Γ F G t l} 
+  {VΓ : [||-v Γ]< wl >}
+  {VF : [Γ ||-v<l> F | VΓ]< wl >}
+  (VΠFG : [Γ ||-v<l> tProd F G | VΓ]< wl >)
+  (Vt : [Γ ||-v<l> t : F | VΓ | VF]< wl >)
   (Δ : context) (σ : nat -> term) 
-  (wfΔ : [ |-[ ta ] Δ]) (vσ : [VΓ | Δ ||-v σ : Γ | wfΔ]) :
-  [Δ ||-< l > G[up_term_term σ][t[σ]..]].
+  (wfΔ : [ |-[ ta ] Δ]< wl >) (vσ : [VΓ | Δ ||-v σ : Γ | wfΔ]< wl >) :
+  W[Δ ||-< l > G[up_term_term σ][t[σ]..]]< wl >.
 Proof.
   eapply singleSubstΠ1.
   eapply (validTy VΠFG); tea.
@@ -256,12 +329,12 @@ Qed.
 Lemma singleSubstComm' G t σ : G[t..][σ] = G[up_term_term σ][t[σ]..].
 Proof. now asimpl. Qed.
 
-Lemma substSΠ {Γ F G t l} 
-  {VΓ : [||-v Γ]}
-  {VF : [Γ ||-v<l> F | VΓ]}
-  (VΠFG : [Γ ||-v<l> tProd F G | VΓ])
-  (Vt : [Γ ||-v<l> t : F | VΓ | VF]) :
-  [Γ ||-v<l> G[t..] | VΓ].
+Lemma substSΠ {wl Γ F G t l} 
+  {VΓ : [||-v Γ]< wl >}
+  {VF : [Γ ||-v<l> F | VΓ]< wl >}
+  (VΠFG : [Γ ||-v<l> tProd F G | VΓ]< wl >)
+  (Vt : [Γ ||-v<l> t : F | VΓ | VF]< wl >) :
+  W[Γ ||-v<l> G[t..] | VΓ]< wl >.
 Proof.
   opector; intros.
   - rewrite singleSubstComm'; now eapply substSΠaux.
@@ -277,18 +350,18 @@ Proof.
     now eapply substSΠaux.
 Qed.
 
-Lemma substSΠeq {Γ F F' G G' t u l} 
-  {VΓ : [||-v Γ]}
-  {VF : [Γ ||-v<l> F | VΓ]}
-  {VF' : [Γ ||-v<l> F' | VΓ]}
-  {VΠFG : [Γ ||-v<l> tProd F G | VΓ]}
-  (VΠFG' : [Γ ||-v<l> tProd F' G' | VΓ])
-  (VΠFGeq : [Γ ||-v<l> tProd F G ≅ tProd F' G' | VΓ | VΠFG])
-  (Vt : [Γ ||-v<l> t : F | VΓ | VF]) 
-  (Vu : [Γ ||-v<l> u : F' | VΓ | VF']) 
-  (Vtu : [Γ ||-v<l> t ≅ u : F | VΓ | VF]) 
+Lemma substSΠeq {wl Γ F F' G G' t u l} 
+  {VΓ : [||-v Γ]< wl >}
+  {VF : [Γ ||-v<l> F | VΓ]< wl >}
+  {VF' : [Γ ||-v<l> F' | VΓ]< wl >}
+  {VΠFG : [Γ ||-v<l> tProd F G | VΓ]< wl >}
+  (VΠFG' : [Γ ||-v<l> tProd F' G' | VΓ]< wl >)
+  (VΠFGeq : [Γ ||-v<l> tProd F G ≅ tProd F' G' | VΓ | VΠFG]< wl >)
+  (Vt : [Γ ||-v<l> t : F | VΓ | VF]< wl >) 
+  (Vu : [Γ ||-v<l> u : F' | VΓ | VF']< wl >) 
+  (Vtu : [Γ ||-v<l> t ≅ u : F | VΓ | VF]< wl >) 
   (VGt := substSΠ VΠFG Vt) :
-  [Γ ||-v<l> G[t..] ≅ G'[u..] | VΓ | VGt].
+  [Γ ||-v<l> G[t..] ≅ G'[u..] | VΓ | VGt]< wl >.
 Proof.
   constructor; intros.
   rewrite singleSubstComm'.
